'is_Datacon' -> 'Datacon?'

src/ocaml-output/FStar_Parser_ToSyntax.ml
@@ -397,22 +397,22 @@ end
 []
 end)
 end
-| (FStar_Parser_AST.Wild) | (FStar_Parser_AST.Const (_)) | (FStar_Parser_AST.Var (_)) | (FStar_Parser_AST.Projector (_)) | (FStar_Parser_AST.Name (_)) -> begin
+| (FStar_Parser_AST.Wild) | (FStar_Parser_AST.Const (_)) | (FStar_Parser_AST.Var (_)) | (FStar_Parser_AST.Projector (_)) | (FStar_Parser_AST.Discrim (_)) | (FStar_Parser_AST.Name (_)) -> begin
 []
 end
 | (FStar_Parser_AST.Assign (_, t)) | (FStar_Parser_AST.Requires (t, _)) | (FStar_Parser_AST.Ensures (t, _)) | (FStar_Parser_AST.NamedTyp (_, t)) | (FStar_Parser_AST.Paren (t)) | (FStar_Parser_AST.Ascribed (t, _)) -> begin
 (free_type_vars env t)
 end
-| FStar_Parser_AST.Construct (_65_269, ts) -> begin
-(FStar_List.collect (fun _65_276 -> (match (_65_276) with
-| (t, _65_275) -> begin
+| FStar_Parser_AST.Construct (_65_272, ts) -> begin
+(FStar_List.collect (fun _65_279 -> (match (_65_279) with
+| (t, _65_278) -> begin
 (free_type_vars env t)
 end)) ts)
 end
-| FStar_Parser_AST.Op (_65_278, ts) -> begin
+| FStar_Parser_AST.Op (_65_281, ts) -> begin
 (FStar_List.collect (free_type_vars env) ts)
 end
-| FStar_Parser_AST.App (t1, t2, _65_285) -> begin
+| FStar_Parser_AST.App (t1, t2, _65_288) -> begin
 (let _160_95 = (free_type_vars env t1)
 in (let _160_94 = (free_type_vars env t2)
 in (FStar_List.append _160_95 _160_94)))
@@ -420,8 +420,8 @@ end
 | FStar_Parser_AST.Refine (b, t) -> begin
 (
 
-let _65_294 = (free_type_vars_b env b)
-in (match (_65_294) with
+let _65_297 = (free_type_vars_b env b)
+in (match (_65_297) with
 | (env, f) -> begin
 (let _160_96 = (free_type_vars env t)
 in (FStar_List.append f _160_96))
@@ -430,23 +430,23 @@ end
 | (FStar_Parser_AST.Product (binders, body)) | (FStar_Parser_AST.Sum (binders, body)) -> begin
 (
 
-let _65_310 = (FStar_List.fold_left (fun _65_303 binder -> (match (_65_303) with
+let _65_313 = (FStar_List.fold_left (fun _65_306 binder -> (match (_65_306) with
 | (env, free) -> begin
 (
 
-let _65_307 = (free_type_vars_b env binder)
-in (match (_65_307) with
+let _65_310 = (free_type_vars_b env binder)
+in (match (_65_310) with
 | (env, f) -> begin
 ((env), ((FStar_List.append f free)))
 end))
 end)) ((env), ([])) binders)
-in (match (_65_310) with
+in (match (_65_313) with
 | (env, free) -> begin
 (let _160_99 = (free_type_vars env body)
 in (FStar_List.append free _160_99))
 end))
 end
-| FStar_Parser_AST.Project (t, _65_313) -> begin
+| FStar_Parser_AST.Project (t, _65_316) -> begin
 (free_type_vars env t)
 end
 | (FStar_Parser_AST.Abs (_)) | (FStar_Parser_AST.Let (_)) | (FStar_Parser_AST.LetOpen (_)) | (FStar_Parser_AST.If (_)) | (FStar_Parser_AST.QForall (_)) | (FStar_Parser_AST.QExists (_)) | (FStar_Parser_AST.Record (_)) | (FStar_Parser_AST.Match (_)) | (FStar_Parser_AST.TryWith (_)) | (FStar_Parser_AST.Seq (_)) -> begin
@@ -464,7 +464,7 @@ end
 | FStar_Parser_AST.Construct (l, args') -> begin
 (({FStar_Parser_AST.tm = FStar_Parser_AST.Name (l); FStar_Parser_AST.range = t.FStar_Parser_AST.range; FStar_Parser_AST.level = t.FStar_Parser_AST.level}), ((FStar_List.append args' args)))
 end
-| _65_360 -> begin
+| _65_363 -> begin
 ((t), (args))
 end))
 in (aux [] t)))
@@ -507,10 +507,10 @@ in (
 
 let t = (match ((let _160_125 = (unparen t)
 in _160_125.FStar_Parser_AST.tm)) with
-| FStar_Parser_AST.Product (_65_373) -> begin
+| FStar_Parser_AST.Product (_65_376) -> begin
 t
 end
-| _65_376 -> begin
+| _65_379 -> begin
 (FStar_Parser_AST.mk_term (FStar_Parser_AST.App ((((FStar_Parser_AST.mk_term (FStar_Parser_AST.Name (FStar_Syntax_Const.effect_Tot_lid)) t.FStar_Parser_AST.range t.FStar_Parser_AST.level)), (t), (FStar_Parser_AST.Nothing)))) t.FStar_Parser_AST.range t.FStar_Parser_AST.level)
 end)
 in (
@@ -524,7 +524,7 @@ let rec uncurry : FStar_Parser_AST.binder Prims.list  ->  FStar_Parser_AST.term 
 | FStar_Parser_AST.Product (binders, t) -> begin
 (uncurry (FStar_List.append bs binders) t)
 end
-| _65_386 -> begin
+| _65_389 -> begin
 ((bs), (t))
 end))
 
@@ -533,22 +533,22 @@ let rec is_var_pattern : FStar_Parser_AST.pattern  ->  Prims.bool = (fun p -> (m
 | (FStar_Parser_AST.PatWild) | (FStar_Parser_AST.PatTvar (_, _)) | (FStar_Parser_AST.PatVar (_, _)) -> begin
 true
 end
-| FStar_Parser_AST.PatAscribed (p, _65_403) -> begin
+| FStar_Parser_AST.PatAscribed (p, _65_406) -> begin
 (is_var_pattern p)
 end
-| _65_407 -> begin
+| _65_410 -> begin
 false
 end))
 
 
 let rec is_app_pattern : FStar_Parser_AST.pattern  ->  Prims.bool = (fun p -> (match (p.FStar_Parser_AST.pat) with
-| FStar_Parser_AST.PatAscribed (p, _65_411) -> begin
+| FStar_Parser_AST.PatAscribed (p, _65_414) -> begin
 (is_app_pattern p)
 end
-| FStar_Parser_AST.PatApp ({FStar_Parser_AST.pat = FStar_Parser_AST.PatVar (_65_417); FStar_Parser_AST.prange = _65_415}, _65_421) -> begin
+| FStar_Parser_AST.PatApp ({FStar_Parser_AST.pat = FStar_Parser_AST.PatVar (_65_420); FStar_Parser_AST.prange = _65_418}, _65_424) -> begin
 true
 end
-| _65_425 -> begin
+| _65_428 -> begin
 false
 end))
 
@@ -557,7 +557,7 @@ let replace_unit_pattern : FStar_Parser_AST.pattern  ->  FStar_Parser_AST.patter
 | FStar_Parser_AST.PatConst (FStar_Const.Const_unit) -> begin
 (FStar_Parser_AST.mk_pattern (FStar_Parser_AST.PatAscribed ((((FStar_Parser_AST.mk_pattern FStar_Parser_AST.PatWild p.FStar_Parser_AST.prange)), (unit_ty)))) p.FStar_Parser_AST.prange)
 end
-| _65_430 -> begin
+| _65_433 -> begin
 p
 end))
 
@@ -566,21 +566,21 @@ let rec destruct_app_pattern : FStar_Parser_Env.env  ->  Prims.bool  ->  FStar_P
 | FStar_Parser_AST.PatAscribed (p, t) -> begin
 (
 
-let _65_442 = (destruct_app_pattern env is_top_level p)
-in (match (_65_442) with
-| (name, args, _65_441) -> begin
+let _65_445 = (destruct_app_pattern env is_top_level p)
+in (match (_65_445) with
+| (name, args, _65_444) -> begin
 ((name), (args), (Some (t)))
 end))
 end
-| FStar_Parser_AST.PatApp ({FStar_Parser_AST.pat = FStar_Parser_AST.PatVar (id, _65_447); FStar_Parser_AST.prange = _65_444}, args) when is_top_level -> begin
+| FStar_Parser_AST.PatApp ({FStar_Parser_AST.pat = FStar_Parser_AST.PatVar (id, _65_450); FStar_Parser_AST.prange = _65_447}, args) when is_top_level -> begin
 (let _160_143 = (let _160_142 = (FStar_Parser_Env.qualify env id)
 in FStar_Util.Inr (_160_142))
 in ((_160_143), (args), (None)))
 end
-| FStar_Parser_AST.PatApp ({FStar_Parser_AST.pat = FStar_Parser_AST.PatVar (id, _65_458); FStar_Parser_AST.prange = _65_455}, args) -> begin
+| FStar_Parser_AST.PatApp ({FStar_Parser_AST.pat = FStar_Parser_AST.PatVar (id, _65_461); FStar_Parser_AST.prange = _65_458}, args) -> begin
 ((FStar_Util.Inl (id)), (args), (None))
 end
-| _65_466 -> begin
+| _65_469 -> begin
 (FStar_All.failwith "Not an app pattern")
 end))
 
@@ -609,14 +609,14 @@ end))
 
 
 let ___LocalBinder____0 = (fun projectee -> (match (projectee) with
-| LocalBinder (_65_469) -> begin
-_65_469
+| LocalBinder (_65_472) -> begin
+_65_472
 end))
 
 
 let ___LetBinder____0 = (fun projectee -> (match (projectee) with
-| LetBinder (_65_472) -> begin
-_65_472
+| LetBinder (_65_475) -> begin
+_65_475
 end))
 
 
@@ -624,7 +624,7 @@ let binder_of_bnd : bnd  ->  (FStar_Syntax_Syntax.bv * FStar_Syntax_Syntax.aqual
 | LocalBinder (a, aq) -> begin
 ((a), (aq))
 end
-| _65_479 -> begin
+| _65_482 -> begin
 (FStar_All.failwith "Impossible")
 end))
 
@@ -637,13 +637,13 @@ end
 | (Some (a), k) -> begin
 (
 
-let _65_492 = (FStar_Parser_Env.push_bv env a)
-in (match (_65_492) with
+let _65_495 = (FStar_Parser_Env.push_bv env a)
+in (match (_65_495) with
 | (env, a) -> begin
 (((((
 
-let _65_493 = a
-in {FStar_Syntax_Syntax.ppname = _65_493.FStar_Syntax_Syntax.ppname; FStar_Syntax_Syntax.index = _65_493.FStar_Syntax_Syntax.index; FStar_Syntax_Syntax.sort = k})), ((trans_aqual imp)))), (env))
+let _65_496 = a
+in {FStar_Syntax_Syntax.ppname = _65_496.FStar_Syntax_Syntax.ppname; FStar_Syntax_Syntax.index = _65_496.FStar_Syntax_Syntax.index; FStar_Syntax_Syntax.sort = k})), ((trans_aqual imp)))), (env))
 end))
 end))
 
@@ -656,7 +656,7 @@ type lenv_t =
 FStar_Syntax_Syntax.bv Prims.list
 
 
-let mk_lb : (FStar_Syntax_Syntax.lbname * FStar_Syntax_Syntax.typ * FStar_Syntax_Syntax.term)  ->  FStar_Syntax_Syntax.letbinding = (fun _65_498 -> (match (_65_498) with
+let mk_lb : (FStar_Syntax_Syntax.lbname * FStar_Syntax_Syntax.typ * FStar_Syntax_Syntax.term)  ->  FStar_Syntax_Syntax.letbinding = (fun _65_501 -> (match (_65_501) with
 | (n, t, e) -> begin
 {FStar_Syntax_Syntax.lbname = n; FStar_Syntax_Syntax.lbunivs = []; FStar_Syntax_Syntax.lbtyp = t; FStar_Syntax_Syntax.lbeff = FStar_Syntax_Const.effect_ALL_lid; FStar_Syntax_Syntax.lbdef = e}
 end))
@@ -708,7 +708,7 @@ let is_special_effect_combinator : Prims.string  ->  Prims.bool = (fun _65_8 -> 
 | ("repr") | ("post") | ("pre") | ("wp") -> begin
 true
 end
-| _65_515 -> begin
+| _65_518 -> begin
 false
 end))
 
@@ -724,9 +724,9 @@ end
 | FStar_Syntax_Syntax.Pat_var (x) -> begin
 (FStar_Util.set_add x FStar_Syntax_Syntax.no_names)
 end
-| FStar_Syntax_Syntax.Pat_cons (_65_535, pats) -> begin
-(FStar_All.pipe_right pats (FStar_List.fold_left (fun out _65_543 -> (match (_65_543) with
-| (p, _65_542) -> begin
+| FStar_Syntax_Syntax.Pat_cons (_65_538, pats) -> begin
+(FStar_All.pipe_right pats (FStar_List.fold_left (fun out _65_546 -> (match (_65_546) with
+| (p, _65_545) -> begin
 (let _160_269 = (pat_vars p)
 in (FStar_Util.set_union out _160_269))
 end)) FStar_Syntax_Syntax.no_names))
@@ -750,11 +750,11 @@ end))
 in (pat_vars p)))
 in (
 
-let _65_566 = (match (((is_mut), (p.FStar_Parser_AST.pat))) with
+let _65_569 = (match (((is_mut), (p.FStar_Parser_AST.pat))) with
 | ((false, _)) | ((true, FStar_Parser_AST.PatVar (_))) -> begin
 ()
 end
-| (true, _65_564) -> begin
+| (true, _65_567) -> begin
 (Prims.raise (FStar_Syntax_Syntax.Error ((("let-mutable is for variables only"), (p.FStar_Parser_AST.prange)))))
 end)
 in (
@@ -770,11 +770,11 @@ let resolvex = (fun l e x -> (match ((FStar_All.pipe_right l (FStar_Util.find_op
 | Some (y) -> begin
 ((l), (e), (y))
 end
-| _65_577 -> begin
+| _65_580 -> begin
 (
 
-let _65_580 = (push_bv_maybe_mut e x)
-in (match (_65_580) with
+let _65_583 = (push_bv_maybe_mut e x)
+in (match (_65_583) with
 | (e, x) -> begin
 (((x)::l), (e), (x))
 end))
@@ -785,11 +785,11 @@ let resolvea = (fun l e a -> (match ((FStar_All.pipe_right l (FStar_Util.find_op
 | Some (b) -> begin
 ((l), (e), (b))
 end
-| _65_589 -> begin
+| _65_592 -> begin
 (
 
-let _65_592 = (push_bv_maybe_mut e a)
-in (match (_65_592) with
+let _65_595 = (push_bv_maybe_mut e a)
+in (match (_65_595) with
 | (e, a) -> begin
 (((a)::l), (e), (a))
 end))
@@ -817,22 +817,22 @@ end
 | FStar_Parser_AST.PatOr ((p)::ps) -> begin
 (
 
-let _65_616 = (aux loc env p)
-in (match (_65_616) with
-| (loc, env, var, p, _65_615) -> begin
+let _65_619 = (aux loc env p)
+in (match (_65_619) with
+| (loc, env, var, p, _65_618) -> begin
 (
 
-let _65_633 = (FStar_List.fold_left (fun _65_620 p -> (match (_65_620) with
+let _65_636 = (FStar_List.fold_left (fun _65_623 p -> (match (_65_623) with
 | (loc, env, ps) -> begin
 (
 
-let _65_629 = (aux loc env p)
-in (match (_65_629) with
-| (loc, env, _65_625, p, _65_628) -> begin
+let _65_632 = (aux loc env p)
+in (match (_65_632) with
+| (loc, env, _65_628, p, _65_631) -> begin
 ((loc), (env), ((p)::ps))
 end))
 end)) ((loc), (env), ([])) ps)
-in (match (_65_633) with
+in (match (_65_636) with
 | (loc, env, ps) -> begin
 (
 
@@ -844,13 +844,13 @@ end
 | FStar_Parser_AST.PatAscribed (p, t) -> begin
 (
 
-let _65_644 = (aux loc env p)
-in (match (_65_644) with
+let _65_647 = (aux loc env p)
+in (match (_65_647) with
 | (loc, env', binder, p, imp) -> begin
 (
 
 let binder = (match (binder) with
-| LetBinder (_65_646) -> begin
+| LetBinder (_65_649) -> begin
 (FStar_All.failwith "impossible")
 end
 | LocalBinder (x, aq) -> begin
@@ -860,8 +860,8 @@ let t = (let _160_308 = (close_fun env t)
 in (desugar_term env _160_308))
 in LocalBinder ((((
 
-let _65_653 = x
-in {FStar_Syntax_Syntax.ppname = _65_653.FStar_Syntax_Syntax.ppname; FStar_Syntax_Syntax.index = _65_653.FStar_Syntax_Syntax.index; FStar_Syntax_Syntax.sort = t})), (aq))))
+let _65_656 = x
+in {FStar_Syntax_Syntax.ppname = _65_656.FStar_Syntax_Syntax.ppname; FStar_Syntax_Syntax.index = _65_656.FStar_Syntax_Syntax.index; FStar_Syntax_Syntax.sort = t})), (aq))))
 end)
 in ((loc), (env'), (binder), (p), (imp)))
 end))
@@ -889,8 +889,8 @@ in (
 let aq = (trans_aqual aq)
 in (
 
-let _65_672 = (resolvex loc env x)
-in (match (_65_672) with
+let _65_675 = (resolvex loc env x)
+in (match (_65_675) with
 | (loc, env, xbv) -> begin
 (let _160_311 = (FStar_All.pipe_left pos (FStar_Syntax_Syntax.Pat_var (xbv)))
 in ((loc), (env), (LocalBinder (((xbv), (aq)))), (_160_311), (imp)))
@@ -906,20 +906,20 @@ let x = (FStar_Syntax_Syntax.new_bv (Some (p.FStar_Parser_AST.prange)) FStar_Syn
 in (let _160_312 = (FStar_All.pipe_left pos (FStar_Syntax_Syntax.Pat_cons (((l), ([])))))
 in ((loc), (env), (LocalBinder (((x), (None)))), (_160_312), (false)))))
 end
-| FStar_Parser_AST.PatApp ({FStar_Parser_AST.pat = FStar_Parser_AST.PatName (l); FStar_Parser_AST.prange = _65_678}, args) -> begin
+| FStar_Parser_AST.PatApp ({FStar_Parser_AST.pat = FStar_Parser_AST.PatName (l); FStar_Parser_AST.prange = _65_681}, args) -> begin
 (
 
-let _65_700 = (FStar_List.fold_right (fun arg _65_689 -> (match (_65_689) with
+let _65_703 = (FStar_List.fold_right (fun arg _65_692 -> (match (_65_692) with
 | (loc, env, args) -> begin
 (
 
-let _65_696 = (aux loc env arg)
-in (match (_65_696) with
-| (loc, env, _65_693, arg, imp) -> begin
+let _65_699 = (aux loc env arg)
+in (match (_65_699) with
+| (loc, env, _65_696, arg, imp) -> begin
 ((loc), (env), ((((arg), (imp)))::args))
 end))
 end)) args ((loc), (env), ([])))
-in (match (_65_700) with
+in (match (_65_703) with
 | (loc, env, args) -> begin
 (
 
@@ -931,23 +931,23 @@ in (let _160_315 = (FStar_All.pipe_left pos (FStar_Syntax_Syntax.Pat_cons (((l),
 in ((loc), (env), (LocalBinder (((x), (None)))), (_160_315), (false)))))
 end))
 end
-| FStar_Parser_AST.PatApp (_65_704) -> begin
+| FStar_Parser_AST.PatApp (_65_707) -> begin
 (Prims.raise (FStar_Syntax_Syntax.Error ((("Unexpected pattern"), (p.FStar_Parser_AST.prange)))))
 end
 | FStar_Parser_AST.PatList (pats) -> begin
 (
 
-let _65_724 = (FStar_List.fold_right (fun pat _65_712 -> (match (_65_712) with
+let _65_727 = (FStar_List.fold_right (fun pat _65_715 -> (match (_65_715) with
 | (loc, env, pats) -> begin
 (
 
-let _65_720 = (aux loc env pat)
-in (match (_65_720) with
-| (loc, env, _65_716, pat, _65_719) -> begin
+let _65_723 = (aux loc env pat)
+in (match (_65_723) with
+| (loc, env, _65_719, pat, _65_722) -> begin
 ((loc), (env), ((pat)::pats))
 end))
 end)) pats ((loc), (env), ([])))
-in (match (_65_724) with
+in (match (_65_727) with
 | (loc, env, pats) -> begin
 (
 
@@ -973,17 +973,17 @@ end
 | FStar_Parser_AST.PatTuple (args, dep) -> begin
 (
 
-let _65_750 = (FStar_List.fold_left (fun _65_737 p -> (match (_65_737) with
+let _65_753 = (FStar_List.fold_left (fun _65_740 p -> (match (_65_740) with
 | (loc, env, pats) -> begin
 (
 
-let _65_746 = (aux loc env p)
-in (match (_65_746) with
-| (loc, env, _65_742, pat, _65_745) -> begin
+let _65_749 = (aux loc env p)
+in (match (_65_749) with
+| (loc, env, _65_745, pat, _65_748) -> begin
 ((loc), (env), ((((pat), (false)))::pats))
 end))
 end)) ((loc), (env), ([])) args)
-in (match (_65_750) with
+in (match (_65_753) with
 | (loc, env, args) -> begin
 (
 
@@ -997,16 +997,16 @@ end else begin
 end
 in (
 
-let _65_756 = (FStar_Parser_Env.fail_or env (FStar_Parser_Env.try_lookup_lid env) l)
-in (match (_65_756) with
-| (constr, _65_755) -> begin
+let _65_759 = (FStar_Parser_Env.fail_or env (FStar_Parser_Env.try_lookup_lid env) l)
+in (match (_65_759) with
+| (constr, _65_758) -> begin
 (
 
 let l = (match (constr.FStar_Syntax_Syntax.n) with
 | FStar_Syntax_Syntax.Tm_fvar (fv) -> begin
 fv
 end
-| _65_760 -> begin
+| _65_763 -> begin
 (FStar_All.failwith "impossible")
 end)
 in (
@@ -1023,33 +1023,33 @@ end
 | FStar_Parser_AST.PatRecord (fields) -> begin
 (
 
-let _65_770 = (FStar_List.hd fields)
-in (match (_65_770) with
-| (f, _65_769) -> begin
+let _65_773 = (FStar_List.hd fields)
+in (match (_65_773) with
+| (f, _65_772) -> begin
 (
 
-let _65_774 = (FStar_Parser_Env.fail_or env (FStar_Parser_Env.try_lookup_record_by_field_name env) f)
-in (match (_65_774) with
-| (record, _65_773) -> begin
+let _65_777 = (FStar_Parser_Env.fail_or env (FStar_Parser_Env.try_lookup_record_by_field_name env) f)
+in (match (_65_777) with
+| (record, _65_776) -> begin
 (
 
-let fields = (FStar_All.pipe_right fields (FStar_List.map (fun _65_777 -> (match (_65_777) with
+let fields = (FStar_All.pipe_right fields (FStar_List.map (fun _65_780 -> (match (_65_780) with
 | (f, p) -> begin
 (let _160_333 = (FStar_Parser_Env.fail_or env (FStar_Parser_Env.qualify_field_to_record env record) f)
 in ((_160_333), (p)))
 end))))
 in (
 
-let args = (FStar_All.pipe_right record.FStar_Parser_Env.fields (FStar_List.map (fun _65_782 -> (match (_65_782) with
-| (f, _65_781) -> begin
-(match ((FStar_All.pipe_right fields (FStar_List.tryFind (fun _65_786 -> (match (_65_786) with
-| (g, _65_785) -> begin
+let args = (FStar_All.pipe_right record.FStar_Parser_Env.fields (FStar_List.map (fun _65_785 -> (match (_65_785) with
+| (f, _65_784) -> begin
+(match ((FStar_All.pipe_right fields (FStar_List.tryFind (fun _65_789 -> (match (_65_789) with
+| (g, _65_788) -> begin
 (FStar_Ident.lid_equals f g)
 end))))) with
 | None -> begin
 (FStar_Parser_AST.mk_pattern FStar_Parser_AST.PatWild p.FStar_Parser_AST.prange)
 end
-| Some (_65_789, p) -> begin
+| Some (_65_792, p) -> begin
 p
 end)
 end))))
@@ -1058,26 +1058,26 @@ in (
 let app = (FStar_Parser_AST.mk_pattern (FStar_Parser_AST.PatApp ((((FStar_Parser_AST.mk_pattern (FStar_Parser_AST.PatName (record.FStar_Parser_Env.constrname)) p.FStar_Parser_AST.prange)), (args)))) p.FStar_Parser_AST.prange)
 in (
 
-let _65_801 = (aux loc env app)
-in (match (_65_801) with
-| (env, e, b, p, _65_800) -> begin
+let _65_804 = (aux loc env app)
+in (match (_65_804) with
+| (env, e, b, p, _65_803) -> begin
 (
 
 let p = (match (p.FStar_Syntax_Syntax.v) with
 | FStar_Syntax_Syntax.Pat_cons (fv, args) -> begin
 (let _160_342 = (let _160_341 = (let _160_340 = (
 
-let _65_806 = fv
+let _65_809 = fv
 in (let _160_339 = (let _160_338 = (let _160_337 = (let _160_336 = (FStar_All.pipe_right record.FStar_Parser_Env.fields (FStar_List.map Prims.fst))
 in ((record.FStar_Parser_Env.typename), (_160_336)))
 in FStar_Syntax_Syntax.Record_ctor (_160_337))
 in Some (_160_338))
-in {FStar_Syntax_Syntax.fv_name = _65_806.FStar_Syntax_Syntax.fv_name; FStar_Syntax_Syntax.fv_delta = _65_806.FStar_Syntax_Syntax.fv_delta; FStar_Syntax_Syntax.fv_qual = _160_339}))
+in {FStar_Syntax_Syntax.fv_name = _65_809.FStar_Syntax_Syntax.fv_name; FStar_Syntax_Syntax.fv_delta = _65_809.FStar_Syntax_Syntax.fv_delta; FStar_Syntax_Syntax.fv_qual = _160_339}))
 in ((_160_340), (args)))
 in FStar_Syntax_Syntax.Pat_cons (_160_341))
 in (FStar_All.pipe_left pos _160_342))
 end
-| _65_809 -> begin
+| _65_812 -> begin
 p
 end)
 in ((env), (e), (b), (p), (false)))
@@ -1087,12 +1087,12 @@ end))
 end))))
 in (
 
-let _65_818 = (aux [] env p)
-in (match (_65_818) with
-| (_65_812, env, b, p, _65_817) -> begin
+let _65_821 = (aux [] env p)
+in (match (_65_821) with
+| (_65_815, env, b, p, _65_820) -> begin
 (
 
-let _65_819 = (let _160_343 = (check_linear_pattern_variables p)
+let _65_822 = (let _160_343 = (check_linear_pattern_variables p)
 in (FStar_All.pipe_left Prims.ignore _160_343))
 in ((env), (b), (p)))
 end)))))))))
@@ -1109,24 +1109,24 @@ in if top then begin
 in (FStar_Ident.id_of_text _160_353))
 in (mklet _160_354))
 end
-| FStar_Parser_AST.PatVar (x, _65_831) -> begin
+| FStar_Parser_AST.PatVar (x, _65_834) -> begin
 (mklet x)
 end
-| FStar_Parser_AST.PatAscribed ({FStar_Parser_AST.pat = FStar_Parser_AST.PatVar (x, _65_838); FStar_Parser_AST.prange = _65_835}, t) -> begin
+| FStar_Parser_AST.PatAscribed ({FStar_Parser_AST.pat = FStar_Parser_AST.PatVar (x, _65_841); FStar_Parser_AST.prange = _65_838}, t) -> begin
 (let _160_358 = (let _160_357 = (let _160_356 = (FStar_Parser_Env.qualify env x)
 in (let _160_355 = (desugar_term env t)
 in ((_160_356), (_160_355))))
 in LetBinder (_160_357))
 in ((env), (_160_358), (None)))
 end
-| _65_846 -> begin
+| _65_849 -> begin
 (Prims.raise (FStar_Syntax_Syntax.Error ((("Unexpected pattern at the top-level"), (p.FStar_Parser_AST.prange)))))
 end)
 end else begin
 (
 
-let _65_850 = (desugar_data_pat env p is_mut)
-in (match (_65_850) with
+let _65_853 = (desugar_data_pat env p is_mut)
+in (match (_65_853) with
 | (env, binder, p) -> begin
 (
 
@@ -1134,18 +1134,18 @@ let p = (match (p.FStar_Syntax_Syntax.v) with
 | (FStar_Syntax_Syntax.Pat_var (_)) | (FStar_Syntax_Syntax.Pat_wild (_)) -> begin
 None
 end
-| _65_858 -> begin
+| _65_861 -> begin
 Some (p)
 end)
 in ((env), (binder), (p)))
 end))
 end))
 and desugar_binding_pat : FStar_Parser_Env.env  ->  FStar_Parser_AST.pattern  ->  (env_t * bnd * FStar_Syntax_Syntax.pat Prims.option) = (fun env p -> (desugar_binding_pat_maybe_top false env p false))
-and desugar_match_pat_maybe_top : Prims.bool  ->  FStar_Parser_Env.env  ->  FStar_Parser_AST.pattern  ->  (env_t * FStar_Syntax_Syntax.pat) = (fun _65_862 env pat -> (
+and desugar_match_pat_maybe_top : Prims.bool  ->  FStar_Parser_Env.env  ->  FStar_Parser_AST.pattern  ->  (env_t * FStar_Syntax_Syntax.pat) = (fun _65_865 env pat -> (
 
-let _65_870 = (desugar_data_pat env pat false)
-in (match (_65_870) with
-| (env, _65_868, pat) -> begin
+let _65_873 = (desugar_data_pat env pat false)
+in (match (_65_873) with
+| (env, _65_871, pat) -> begin
 ((env), (pat))
 end)))
 and desugar_match_pat : FStar_Parser_Env.env  ->  FStar_Parser_AST.pattern  ->  (env_t * FStar_Syntax_Syntax.pat) = (fun env p -> (desugar_match_pat_maybe_top false env p))
@@ -1153,17 +1153,17 @@ and desugar_term : FStar_Parser_Env.env  ->  FStar_Parser_AST.term  ->  FStar_Sy
 
 let env = (
 
-let _65_875 = env
-in {FStar_Parser_Env.curmodule = _65_875.FStar_Parser_Env.curmodule; FStar_Parser_Env.curmonad = _65_875.FStar_Parser_Env.curmonad; FStar_Parser_Env.modules = _65_875.FStar_Parser_Env.modules; FStar_Parser_Env.open_namespaces = _65_875.FStar_Parser_Env.open_namespaces; FStar_Parser_Env.modul_abbrevs = _65_875.FStar_Parser_Env.modul_abbrevs; FStar_Parser_Env.sigaccum = _65_875.FStar_Parser_Env.sigaccum; FStar_Parser_Env.localbindings = _65_875.FStar_Parser_Env.localbindings; FStar_Parser_Env.recbindings = _65_875.FStar_Parser_Env.recbindings; FStar_Parser_Env.sigmap = _65_875.FStar_Parser_Env.sigmap; FStar_Parser_Env.default_result_effect = _65_875.FStar_Parser_Env.default_result_effect; FStar_Parser_Env.iface = _65_875.FStar_Parser_Env.iface; FStar_Parser_Env.admitted_iface = _65_875.FStar_Parser_Env.admitted_iface; FStar_Parser_Env.expect_typ = false})
+let _65_878 = env
+in {FStar_Parser_Env.curmodule = _65_878.FStar_Parser_Env.curmodule; FStar_Parser_Env.curmonad = _65_878.FStar_Parser_Env.curmonad; FStar_Parser_Env.modules = _65_878.FStar_Parser_Env.modules; FStar_Parser_Env.open_namespaces = _65_878.FStar_Parser_Env.open_namespaces; FStar_Parser_Env.modul_abbrevs = _65_878.FStar_Parser_Env.modul_abbrevs; FStar_Parser_Env.sigaccum = _65_878.FStar_Parser_Env.sigaccum; FStar_Parser_Env.localbindings = _65_878.FStar_Parser_Env.localbindings; FStar_Parser_Env.recbindings = _65_878.FStar_Parser_Env.recbindings; FStar_Parser_Env.sigmap = _65_878.FStar_Parser_Env.sigmap; FStar_Parser_Env.default_result_effect = _65_878.FStar_Parser_Env.default_result_effect; FStar_Parser_Env.iface = _65_878.FStar_Parser_Env.iface; FStar_Parser_Env.admitted_iface = _65_878.FStar_Parser_Env.admitted_iface; FStar_Parser_Env.expect_typ = false})
 in (desugar_term_maybe_top false env e)))
 and desugar_typ : FStar_Parser_Env.env  ->  FStar_Parser_AST.term  ->  FStar_Syntax_Syntax.term = (fun env e -> (
 
 let env = (
 
-let _65_880 = env
-in {FStar_Parser_Env.curmodule = _65_880.FStar_Parser_Env.curmodule; FStar_Parser_Env.curmonad = _65_880.FStar_Parser_Env.curmonad; FStar_Parser_Env.modules = _65_880.FStar_Parser_Env.modules; FStar_Parser_Env.open_namespaces = _65_880.FStar_Parser_Env.open_namespaces; FStar_Parser_Env.modul_abbrevs = _65_880.FStar_Parser_Env.modul_abbrevs; FStar_Parser_Env.sigaccum = _65_880.FStar_Parser_Env.sigaccum; FStar_Parser_Env.localbindings = _65_880.FStar_Parser_Env.localbindings; FStar_Parser_Env.recbindings = _65_880.FStar_Parser_Env.recbindings; FStar_Parser_Env.sigmap = _65_880.FStar_Parser_Env.sigmap; FStar_Parser_Env.default_result_effect = _65_880.FStar_Parser_Env.default_result_effect; FStar_Parser_Env.iface = _65_880.FStar_Parser_Env.iface; FStar_Parser_Env.admitted_iface = _65_880.FStar_Parser_Env.admitted_iface; FStar_Parser_Env.expect_typ = true})
+let _65_883 = env
+in {FStar_Parser_Env.curmodule = _65_883.FStar_Parser_Env.curmodule; FStar_Parser_Env.curmonad = _65_883.FStar_Parser_Env.curmonad; FStar_Parser_Env.modules = _65_883.FStar_Parser_Env.modules; FStar_Parser_Env.open_namespaces = _65_883.FStar_Parser_Env.open_namespaces; FStar_Parser_Env.modul_abbrevs = _65_883.FStar_Parser_Env.modul_abbrevs; FStar_Parser_Env.sigaccum = _65_883.FStar_Parser_Env.sigaccum; FStar_Parser_Env.localbindings = _65_883.FStar_Parser_Env.localbindings; FStar_Parser_Env.recbindings = _65_883.FStar_Parser_Env.recbindings; FStar_Parser_Env.sigmap = _65_883.FStar_Parser_Env.sigmap; FStar_Parser_Env.default_result_effect = _65_883.FStar_Parser_Env.default_result_effect; FStar_Parser_Env.iface = _65_883.FStar_Parser_Env.iface; FStar_Parser_Env.admitted_iface = _65_883.FStar_Parser_Env.admitted_iface; FStar_Parser_Env.expect_typ = true})
 in (desugar_term_maybe_top false env e)))
-and desugar_machine_integer : FStar_Parser_Env.env  ->  Prims.string  ->  (FStar_Const.signedness * FStar_Const.width)  ->  FStar_Range.range  ->  (FStar_Syntax_Syntax.term', FStar_Syntax_Syntax.term') FStar_Syntax_Syntax.syntax = (fun env repr _65_887 range -> (match (_65_887) with
+and desugar_machine_integer : FStar_Parser_Env.env  ->  Prims.string  ->  (FStar_Const.signedness * FStar_Const.width)  ->  FStar_Range.range  ->  (FStar_Syntax_Syntax.term', FStar_Syntax_Syntax.term') FStar_Syntax_Syntax.syntax = (fun env repr _65_890 range -> (match (_65_890) with
 | (signedness, width) -> begin
 (
 
@@ -1217,8 +1217,8 @@ in (FStar_Syntax_Syntax.mk _160_379 None range))))))
 end))
 and desugar_name : (FStar_Syntax_Syntax.term'  ->  FStar_Syntax_Syntax.term)  ->  (FStar_Syntax_Syntax.term  ->  (FStar_Syntax_Syntax.term', FStar_Syntax_Syntax.term') FStar_Syntax_Syntax.syntax)  ->  env_t  ->  FStar_Ident.lid  ->  FStar_Syntax_Syntax.term = (fun mk setpos env l -> (
 
-let _65_910 = (FStar_Parser_Env.fail_or env (FStar_Parser_Env.try_lookup_lid env) l)
-in (match (_65_910) with
+let _65_913 = (FStar_Parser_Env.fail_or env (FStar_Parser_Env.try_lookup_lid env) l)
+in (match (_65_913) with
 | (tm, mut) -> begin
 (
 
@@ -1239,14 +1239,14 @@ in (
 
 let setpos = (fun e -> (
 
-let _65_919 = e
-in {FStar_Syntax_Syntax.n = _65_919.FStar_Syntax_Syntax.n; FStar_Syntax_Syntax.tk = _65_919.FStar_Syntax_Syntax.tk; FStar_Syntax_Syntax.pos = top.FStar_Parser_AST.range; FStar_Syntax_Syntax.vars = _65_919.FStar_Syntax_Syntax.vars}))
+let _65_922 = e
+in {FStar_Syntax_Syntax.n = _65_922.FStar_Syntax_Syntax.n; FStar_Syntax_Syntax.tk = _65_922.FStar_Syntax_Syntax.tk; FStar_Syntax_Syntax.pos = top.FStar_Parser_AST.range; FStar_Syntax_Syntax.vars = _65_922.FStar_Syntax_Syntax.vars}))
 in (match ((let _160_400 = (unparen top)
 in _160_400.FStar_Parser_AST.tm)) with
 | FStar_Parser_AST.Wild -> begin
 (setpos FStar_Syntax_Syntax.tun)
 end
-| FStar_Parser_AST.Labeled (_65_923) -> begin
+| FStar_Parser_AST.Labeled (_65_926) -> begin
 (desugar_formula env top)
 end
 | FStar_Parser_AST.Requires (t, lopt) -> begin
@@ -1264,7 +1264,7 @@ end
 | FStar_Parser_AST.Op ("=!=", args) -> begin
 (desugar_term env (FStar_Parser_AST.mk_term (FStar_Parser_AST.Op ((("~"), (((FStar_Parser_AST.mk_term (FStar_Parser_AST.Op ((("=="), (args)))) top.FStar_Parser_AST.range top.FStar_Parser_AST.level))::[])))) top.FStar_Parser_AST.range top.FStar_Parser_AST.level))
 end
-| FStar_Parser_AST.Op ("*", (_65_949)::(_65_947)::[]) when (let _160_401 = (op_as_term env (Prims.parse_int "2") top.FStar_Parser_AST.range "*")
+| FStar_Parser_AST.Op ("*", (_65_952)::(_65_950)::[]) when (let _160_401 = (op_as_term env (Prims.parse_int "2") top.FStar_Parser_AST.range "*")
 in (FStar_All.pipe_right _160_401 FStar_Option.isNone)) -> begin
 (
 
@@ -1273,7 +1273,7 @@ let rec flatten = (fun t -> (match (t.FStar_Parser_AST.tm) with
 (let _160_404 = (flatten t1)
 in (FStar_List.append _160_404 ((t2)::[])))
 end
-| _65_962 -> begin
+| _65_965 -> begin
 (t)::[]
 end))
 in (
@@ -1284,10 +1284,10 @@ in (FStar_All.pipe_right _160_408 (FStar_List.map (fun t -> (let _160_407 = (des
 in (FStar_Syntax_Syntax.as_arg _160_407))))))
 in (
 
-let _65_968 = (let _160_409 = (FStar_Syntax_Util.mk_tuple_lid (FStar_List.length targs) top.FStar_Parser_AST.range)
+let _65_971 = (let _160_409 = (FStar_Syntax_Util.mk_tuple_lid (FStar_List.length targs) top.FStar_Parser_AST.range)
 in (FStar_Parser_Env.fail_or env (FStar_Parser_Env.try_lookup_lid env) _160_409))
-in (match (_65_968) with
-| (tup, _65_967) -> begin
+in (match (_65_971) with
+| (tup, _65_970) -> begin
 (mk (FStar_Syntax_Syntax.Tm_app (((tup), (targs)))))
 end))))
 end
@@ -1313,22 +1313,22 @@ op
 end
 end)
 end
-| FStar_Parser_AST.Name ({FStar_Ident.ns = _65_986; FStar_Ident.ident = _65_984; FStar_Ident.nsstr = _65_982; FStar_Ident.str = "Type0"}) -> begin
+| FStar_Parser_AST.Name ({FStar_Ident.ns = _65_989; FStar_Ident.ident = _65_987; FStar_Ident.nsstr = _65_985; FStar_Ident.str = "Type0"}) -> begin
 (mk (FStar_Syntax_Syntax.Tm_type (FStar_Syntax_Syntax.U_zero)))
 end
-| FStar_Parser_AST.Name ({FStar_Ident.ns = _65_995; FStar_Ident.ident = _65_993; FStar_Ident.nsstr = _65_991; FStar_Ident.str = "Type"}) -> begin
+| FStar_Parser_AST.Name ({FStar_Ident.ns = _65_998; FStar_Ident.ident = _65_996; FStar_Ident.nsstr = _65_994; FStar_Ident.str = "Type"}) -> begin
 (mk (FStar_Syntax_Syntax.Tm_type (FStar_Syntax_Syntax.U_unknown)))
 end
-| FStar_Parser_AST.Name ({FStar_Ident.ns = _65_1004; FStar_Ident.ident = _65_1002; FStar_Ident.nsstr = _65_1000; FStar_Ident.str = "Effect"}) -> begin
+| FStar_Parser_AST.Name ({FStar_Ident.ns = _65_1007; FStar_Ident.ident = _65_1005; FStar_Ident.nsstr = _65_1003; FStar_Ident.str = "Effect"}) -> begin
 (mk (FStar_Syntax_Syntax.Tm_constant (FStar_Const.Const_effect)))
 end
-| FStar_Parser_AST.Name ({FStar_Ident.ns = _65_1013; FStar_Ident.ident = _65_1011; FStar_Ident.nsstr = _65_1009; FStar_Ident.str = "True"}) -> begin
+| FStar_Parser_AST.Name ({FStar_Ident.ns = _65_1016; FStar_Ident.ident = _65_1014; FStar_Ident.nsstr = _65_1012; FStar_Ident.str = "True"}) -> begin
 (FStar_Syntax_Syntax.fvar (FStar_Ident.set_lid_range FStar_Syntax_Const.true_lid top.FStar_Parser_AST.range) FStar_Syntax_Syntax.Delta_constant None)
 end
-| FStar_Parser_AST.Name ({FStar_Ident.ns = _65_1022; FStar_Ident.ident = _65_1020; FStar_Ident.nsstr = _65_1018; FStar_Ident.str = "False"}) -> begin
+| FStar_Parser_AST.Name ({FStar_Ident.ns = _65_1025; FStar_Ident.ident = _65_1023; FStar_Ident.nsstr = _65_1021; FStar_Ident.str = "False"}) -> begin
 (FStar_Syntax_Syntax.fvar (FStar_Ident.set_lid_range FStar_Syntax_Const.false_lid top.FStar_Parser_AST.range) FStar_Syntax_Syntax.Delta_constant None)
 end
-| FStar_Parser_AST.Projector (eff_name, {FStar_Ident.idText = txt; FStar_Ident.idRange = _65_1027}) when ((is_special_effect_combinator txt) && (FStar_Parser_Env.is_effect_name env eff_name)) -> begin
+| FStar_Parser_AST.Projector (eff_name, {FStar_Ident.idText = txt; FStar_Ident.idRange = _65_1030}) when ((is_special_effect_combinator txt) && (FStar_Parser_Env.is_effect_name env eff_name)) -> begin
 (match ((FStar_Parser_Env.try_lookup_effect_defn env eff_name)) with
 | Some (ed) -> begin
 (let _160_414 = (FStar_Ident.lid_of_path (FStar_Ident.path_of_text (Prims.strcat (FStar_Ident.text_of_lid ed.FStar_Syntax_Syntax.mname) (Prims.strcat "_" txt))) FStar_Range.dummyRange)
@@ -1344,12 +1344,12 @@ end
 let t2 = (desugar_term env t2)
 in (
 
-let _65_1042 = (FStar_Parser_Env.fail_or2 (FStar_Parser_Env.try_lookup_id env) ident)
-in (match (_65_1042) with
+let _65_1045 = (FStar_Parser_Env.fail_or2 (FStar_Parser_Env.try_lookup_id env) ident)
+in (match (_65_1045) with
 | (t1, mut) -> begin
 (
 
-let _65_1043 = if (not (mut)) then begin
+let _65_1046 = if (not (mut)) then begin
 (Prims.raise (FStar_Syntax_Syntax.Error ((("Can only assign to mutable values"), (top.FStar_Parser_AST.range)))))
 end else begin
 ()
@@ -1364,23 +1364,29 @@ end
 (let _160_415 = (FStar_Syntax_Util.mk_field_projector_name_from_ident l i)
 in (desugar_name mk setpos env _160_415))
 end
+| FStar_Parser_AST.Discrim (lid) -> begin
+(
+
+let lid' = (FStar_Syntax_Util.mk_discriminator lid)
+in (desugar_name mk setpos env lid'))
+end
 | FStar_Parser_AST.Construct (l, args) -> begin
 (match ((FStar_Parser_Env.try_lookup_datacon env l)) with
 | Some (head) -> begin
 (
 
-let _65_1060 = (let _160_416 = (mk (FStar_Syntax_Syntax.Tm_fvar (head)))
+let _65_1066 = (let _160_416 = (mk (FStar_Syntax_Syntax.Tm_fvar (head)))
 in ((_160_416), (true)))
-in (match (_65_1060) with
+in (match (_65_1066) with
 | (head, is_data) -> begin
 (match (args) with
 | [] -> begin
 head
 end
-| _65_1063 -> begin
+| _65_1069 -> begin
 (
 
-let args = (FStar_List.map (fun _65_1066 -> (match (_65_1066) with
+let args = (FStar_List.map (fun _65_1072 -> (match (_65_1072) with
 | (t, imp) -> begin
 (
 
@@ -1405,16 +1411,16 @@ end
 | FStar_Parser_AST.Sum (binders, t) -> begin
 (
 
-let _65_1095 = (FStar_List.fold_left (fun _65_1078 b -> (match (_65_1078) with
+let _65_1101 = (FStar_List.fold_left (fun _65_1084 b -> (match (_65_1084) with
 | (env, tparams, typs) -> begin
 (
 
-let _65_1082 = (desugar_binder env b)
-in (match (_65_1082) with
+let _65_1088 = (desugar_binder env b)
+in (match (_65_1088) with
 | (xopt, t) -> begin
 (
 
-let _65_1088 = (match (xopt) with
+let _65_1094 = (match (xopt) with
 | None -> begin
 (let _160_420 = (FStar_Syntax_Syntax.new_bv (Some (top.FStar_Parser_AST.range)) FStar_Syntax_Syntax.tun)
 in ((env), (_160_420)))
@@ -1422,7 +1428,7 @@ end
 | Some (x) -> begin
 (FStar_Parser_Env.push_bv env x)
 end)
-in (match (_65_1088) with
+in (match (_65_1094) with
 | (env, x) -> begin
 (let _160_424 = (let _160_423 = (let _160_422 = (let _160_421 = (no_annot_abs tparams t)
 in (FStar_All.pipe_left FStar_Syntax_Syntax.as_arg _160_421))
@@ -1430,19 +1436,19 @@ in (_160_422)::[])
 in (FStar_List.append typs _160_423))
 in ((env), ((FStar_List.append tparams (((((
 
-let _65_1089 = x
-in {FStar_Syntax_Syntax.ppname = _65_1089.FStar_Syntax_Syntax.ppname; FStar_Syntax_Syntax.index = _65_1089.FStar_Syntax_Syntax.index; FStar_Syntax_Syntax.sort = t})), (None)))::[]))), (_160_424)))
+let _65_1095 = x
+in {FStar_Syntax_Syntax.ppname = _65_1095.FStar_Syntax_Syntax.ppname; FStar_Syntax_Syntax.index = _65_1095.FStar_Syntax_Syntax.index; FStar_Syntax_Syntax.sort = t})), (None)))::[]))), (_160_424)))
 end))
 end))
 end)) ((env), ([]), ([])) (FStar_List.append binders (((FStar_Parser_AST.mk_binder (FStar_Parser_AST.NoName (t)) t.FStar_Parser_AST.range FStar_Parser_AST.Type None))::[])))
-in (match (_65_1095) with
-| (env, _65_1093, targs) -> begin
+in (match (_65_1101) with
+| (env, _65_1099, targs) -> begin
 (
 
-let _65_1099 = (let _160_425 = (FStar_Syntax_Util.mk_dtuple_lid (FStar_List.length targs) top.FStar_Parser_AST.range)
+let _65_1105 = (let _160_425 = (FStar_Syntax_Util.mk_dtuple_lid (FStar_List.length targs) top.FStar_Parser_AST.range)
 in (FStar_Parser_Env.fail_or env (FStar_Parser_Env.try_lookup_lid env) _160_425))
-in (match (_65_1099) with
-| (tup, _65_1098) -> begin
+in (match (_65_1105) with
+| (tup, _65_1104) -> begin
 (FStar_All.pipe_left mk (FStar_Syntax_Syntax.Tm_app (((tup), (targs)))))
 end))
 end))
@@ -1450,8 +1456,8 @@ end
 | FStar_Parser_AST.Product (binders, t) -> begin
 (
 
-let _65_1106 = (uncurry binders t)
-in (match (_65_1106) with
+let _65_1112 = (uncurry binders t)
+in (match (_65_1112) with
 | (bs, t) -> begin
 (
 
@@ -1472,8 +1478,8 @@ in (
 let bb = (desugar_binder mlenv hd)
 in (
 
-let _65_1120 = (as_binder env hd.FStar_Parser_AST.aqual bb)
-in (match (_65_1120) with
+let _65_1126 = (as_binder env hd.FStar_Parser_AST.aqual bb)
+in (match (_65_1126) with
 | (b, env) -> begin
 (aux env ((b)::bs) tl)
 end))))
@@ -1483,15 +1489,15 @@ end))
 end
 | FStar_Parser_AST.Refine (b, f) -> begin
 (match ((desugar_binder env b)) with
-| (None, _65_1127) -> begin
+| (None, _65_1133) -> begin
 (FStar_All.failwith "Missing binder in refinement")
 end
 | b -> begin
 (
 
-let _65_1135 = (as_binder env None b)
-in (match (_65_1135) with
-| ((x, _65_1132), env) -> begin
+let _65_1141 = (as_binder env None b)
+in (match (_65_1141) with
+| ((x, _65_1138), env) -> begin
 (
 
 let f = (desugar_formula env f)
@@ -1506,20 +1512,20 @@ end
 let binders = (FStar_All.pipe_right binders (FStar_List.map replace_unit_pattern))
 in (
 
-let _65_1156 = (FStar_List.fold_left (fun _65_1144 pat -> (match (_65_1144) with
+let _65_1162 = (FStar_List.fold_left (fun _65_1150 pat -> (match (_65_1150) with
 | (env, ftvs) -> begin
 (match (pat.FStar_Parser_AST.pat) with
-| FStar_Parser_AST.PatAscribed (_65_1147, t) -> begin
+| FStar_Parser_AST.PatAscribed (_65_1153, t) -> begin
 (let _160_437 = (let _160_436 = (free_type_vars env t)
 in (FStar_List.append _160_436 ftvs))
 in ((env), (_160_437)))
 end
-| _65_1152 -> begin
+| _65_1158 -> begin
 ((env), (ftvs))
 end)
 end)) ((env), ([])) binders)
-in (match (_65_1156) with
-| (_65_1154, ftv) -> begin
+in (match (_65_1162) with
+| (_65_1160, ftv) -> begin
 (
 
 let ftv = (sort_ftv ftv)
@@ -1554,20 +1560,20 @@ end
 | (p)::rest -> begin
 (
 
-let _65_1180 = (desugar_binding_pat env p)
-in (match (_65_1180) with
+let _65_1186 = (desugar_binding_pat env p)
+in (match (_65_1186) with
 | (env, b, pat) -> begin
 (
 
-let _65_1231 = (match (b) with
-| LetBinder (_65_1182) -> begin
+let _65_1237 = (match (b) with
+| LetBinder (_65_1188) -> begin
 (FStar_All.failwith "Impossible")
 end
 | LocalBinder (x, aq) -> begin
 (
 
 let sc_pat_opt = (match (((pat), (sc_pat_opt))) with
-| (None, _65_1190) -> begin
+| (None, _65_1196) -> begin
 sc_pat_opt
 end
 | (Some (p), None) -> begin
@@ -1577,7 +1583,7 @@ in Some (_160_452))
 end
 | (Some (p), Some (sc, p')) -> begin
 (match (((sc.FStar_Syntax_Syntax.n), (p'.FStar_Syntax_Syntax.v))) with
-| (FStar_Syntax_Syntax.Tm_name (_65_1204), _65_1207) -> begin
+| (FStar_Syntax_Syntax.Tm_name (_65_1210), _65_1213) -> begin
 (
 
 let tup2 = (let _160_453 = (FStar_Syntax_Util.mk_tuple_data_lid (Prims.parse_int "2") top.FStar_Parser_AST.range)
@@ -1599,7 +1605,7 @@ let p = (let _160_462 = (FStar_Range.union_ranges p'.FStar_Syntax_Syntax.p p.FSt
 in (FStar_Syntax_Syntax.withinfo (FStar_Syntax_Syntax.Pat_cons (((tup2), ((((p'), (false)))::(((p), (false)))::[])))) FStar_Syntax_Syntax.tun.FStar_Syntax_Syntax.n _160_462))
 in Some (((sc), (p))))))
 end
-| (FStar_Syntax_Syntax.Tm_app (_65_1213, args), FStar_Syntax_Syntax.Pat_cons (_65_1218, pats)) -> begin
+| (FStar_Syntax_Syntax.Tm_app (_65_1219, args), FStar_Syntax_Syntax.Pat_cons (_65_1224, pats)) -> begin
 (
 
 let tupn = (let _160_463 = (FStar_Syntax_Util.mk_tuple_data_lid ((Prims.parse_int "1") + (FStar_List.length args)) top.FStar_Parser_AST.range)
@@ -1620,13 +1626,13 @@ let p = (let _160_471 = (FStar_Range.union_ranges p'.FStar_Syntax_Syntax.p p.FSt
 in (FStar_Syntax_Syntax.withinfo (FStar_Syntax_Syntax.Pat_cons (((tupn), ((FStar_List.append pats ((((p), (false)))::[])))))) FStar_Syntax_Syntax.tun.FStar_Syntax_Syntax.n _160_471))
 in Some (((sc), (p))))))
 end
-| _65_1227 -> begin
+| _65_1233 -> begin
 (FStar_All.failwith "Impossible")
 end)
 end)
 in ((((x), (aq))), (sc_pat_opt)))
 end)
-in (match (_65_1231) with
+in (match (_65_1237) with
 | (b, sc_pat_opt) -> begin
 (aux env ((b)::bs) sc_pat_opt rest)
 end))
@@ -1635,7 +1641,7 @@ end))
 in (aux env [] None binders))))
 end)))
 end
-| FStar_Parser_AST.App ({FStar_Parser_AST.tm = FStar_Parser_AST.Var (a); FStar_Parser_AST.range = rng; FStar_Parser_AST.level = _65_1233}, phi, _65_1240) when ((FStar_Ident.lid_equals a FStar_Syntax_Const.assert_lid) || (FStar_Ident.lid_equals a FStar_Syntax_Const.assume_lid)) -> begin
+| FStar_Parser_AST.App ({FStar_Parser_AST.tm = FStar_Parser_AST.Var (a); FStar_Parser_AST.range = rng; FStar_Parser_AST.level = _65_1239}, phi, _65_1246) when ((FStar_Ident.lid_equals a FStar_Syntax_Const.assert_lid) || (FStar_Ident.lid_equals a FStar_Syntax_Const.assume_lid)) -> begin
 (
 
 let phi = (desugar_formula env phi)
@@ -1652,7 +1658,7 @@ in ((_160_477), (_160_476))))
 in FStar_Syntax_Syntax.Tm_app (_160_478))
 in (mk _160_479))))
 end
-| FStar_Parser_AST.App (_65_1246) -> begin
+| FStar_Parser_AST.App (_65_1252) -> begin
 (
 
 let rec aux = (fun args e -> (match ((let _160_484 = (unparen e)
@@ -1664,7 +1670,7 @@ let arg = (let _160_485 = (desugar_term env t)
 in (FStar_All.pipe_left (arg_withimp_e imp) _160_485))
 in (aux ((arg)::args) e))
 end
-| _65_1258 -> begin
+| _65_1264 -> begin
 (
 
 let head = (desugar_term env e)
@@ -1693,14 +1699,14 @@ end
 let is_rec = (qual = FStar_Parser_AST.Rec)
 in (
 
-let ds_let_rec_or_app = (fun _65_1281 -> (match (()) with
+let ds_let_rec_or_app = (fun _65_1287 -> (match (()) with
 | () -> begin
 (
 
 let bindings = (((pat), (_snd)))::_tl
 in (
 
-let funs = (FStar_All.pipe_right bindings (FStar_List.map (fun _65_1285 -> (match (_65_1285) with
+let funs = (FStar_All.pipe_right bindings (FStar_List.map (fun _65_1291 -> (match (_65_1291) with
 | (p, def) -> begin
 if (is_app_pattern p) then begin
 (let _160_492 = (destruct_app_pattern env top_level p)
@@ -1711,9 +1717,9 @@ end else begin
 (let _160_493 = (destruct_app_pattern env top_level p)
 in ((_160_493), (def)))
 end
-| _65_1291 -> begin
+| _65_1297 -> begin
 (match (p.FStar_Parser_AST.pat) with
-| FStar_Parser_AST.PatAscribed ({FStar_Parser_AST.pat = FStar_Parser_AST.PatVar (id, _65_1296); FStar_Parser_AST.prange = _65_1293}, t) -> begin
+| FStar_Parser_AST.PatAscribed ({FStar_Parser_AST.pat = FStar_Parser_AST.PatVar (id, _65_1302); FStar_Parser_AST.prange = _65_1299}, t) -> begin
 if top_level then begin
 (let _160_496 = (let _160_495 = (let _160_494 = (FStar_Parser_Env.qualify env id)
 in FStar_Util.Inr (_160_494))
@@ -1723,7 +1729,7 @@ end else begin
 ((((FStar_Util.Inl (id)), ([]), (Some (t)))), (def))
 end
 end
-| FStar_Parser_AST.PatVar (id, _65_1305) -> begin
+| FStar_Parser_AST.PatVar (id, _65_1311) -> begin
 if top_level then begin
 (let _160_499 = (let _160_498 = (let _160_497 = (FStar_Parser_Env.qualify env id)
 in FStar_Util.Inr (_160_497))
@@ -1733,7 +1739,7 @@ end else begin
 ((((FStar_Util.Inl (id)), ([]), (None))), (def))
 end
 end
-| _65_1309 -> begin
+| _65_1315 -> begin
 (Prims.raise (FStar_Syntax_Syntax.Error ((("Unexpected let binding"), (p.FStar_Parser_AST.prange)))))
 end)
 end)
@@ -1741,16 +1747,16 @@ end
 end))))
 in (
 
-let _65_1338 = (FStar_List.fold_left (fun _65_1314 _65_1323 -> (match (((_65_1314), (_65_1323))) with
-| ((env, fnames, rec_bindings), ((f, _65_1317, _65_1319), _65_1322)) -> begin
+let _65_1344 = (FStar_List.fold_left (fun _65_1320 _65_1329 -> (match (((_65_1320), (_65_1329))) with
+| ((env, fnames, rec_bindings), ((f, _65_1323, _65_1325), _65_1328)) -> begin
 (
 
-let _65_1334 = (match (f) with
+let _65_1340 = (match (f) with
 | FStar_Util.Inl (x) -> begin
 (
 
-let _65_1328 = (FStar_Parser_Env.push_bv env x)
-in (match (_65_1328) with
+let _65_1334 = (FStar_Parser_Env.push_bv env x)
+in (match (_65_1334) with
 | (env, xx) -> begin
 (let _160_503 = (let _160_502 = (FStar_Syntax_Syntax.mk_binder xx)
 in (_160_502)::rec_bindings)
@@ -1761,20 +1767,20 @@ end
 (let _160_504 = (FStar_Parser_Env.push_top_level_rec_binding env l.FStar_Ident.ident FStar_Syntax_Syntax.Delta_equational)
 in ((_160_504), (FStar_Util.Inr (l)), (rec_bindings)))
 end)
-in (match (_65_1334) with
+in (match (_65_1340) with
 | (env, lbname, rec_bindings) -> begin
 ((env), ((lbname)::fnames), (rec_bindings))
 end))
 end)) ((env), ([]), ([])) funs)
-in (match (_65_1338) with
+in (match (_65_1344) with
 | (env', fnames, rec_bindings) -> begin
 (
 
 let fnames = (FStar_List.rev fnames)
 in (
 
-let desugar_one_def = (fun env lbname _65_1349 -> (match (_65_1349) with
-| ((_65_1344, args, result_t), def) -> begin
+let desugar_one_def = (fun env lbname _65_1355 -> (match (_65_1355) with
+| ((_65_1350, args, result_t), def) -> begin
 (
 
 let args = (FStar_All.pipe_right args (FStar_List.map replace_unit_pattern))
@@ -1787,7 +1793,7 @@ end
 | Some (t) -> begin
 (
 
-let _65_1358 = if (is_comp_type env t) then begin
+let _65_1364 = if (is_comp_type env t) then begin
 (match ((FStar_All.pipe_right args (FStar_List.tryFind (fun x -> (not ((is_var_pattern x))))))) with
 | None -> begin
 ()
@@ -1807,7 +1813,7 @@ let def = (match (args) with
 | [] -> begin
 def
 end
-| _65_1363 -> begin
+| _65_1369 -> begin
 (FStar_Parser_AST.mk_term (FStar_Parser_AST.un_curry_abs args def) top.FStar_Parser_AST.range top.FStar_Parser_AST.level)
 end)
 in (
@@ -1866,8 +1872,8 @@ t1
 end
 in (
 
-let _65_1384 = (desugar_binding_pat_maybe_top top_level env pat is_mutable)
-in (match (_65_1384) with
+let _65_1390 = (desugar_binding_pat_maybe_top top_level env pat is_mutable)
+in (match (_65_1390) with
 | (env, binder, pat) -> begin
 (
 
@@ -1882,7 +1888,7 @@ let fv = (let _160_524 = (FStar_Syntax_Util.incr_delta_qualifier t1)
 in (FStar_Syntax_Syntax.lid_as_fv l _160_524 None))
 in (FStar_All.pipe_left mk (FStar_Syntax_Syntax.Tm_let (((((false), (({FStar_Syntax_Syntax.lbname = FStar_Util.Inr (fv); FStar_Syntax_Syntax.lbunivs = []; FStar_Syntax_Syntax.lbtyp = t; FStar_Syntax_Syntax.lbeff = FStar_Syntax_Const.effect_ALL_lid; FStar_Syntax_Syntax.lbdef = t1})::[]))), (body)))))))
 end
-| LocalBinder (x, _65_1393) -> begin
+| LocalBinder (x, _65_1399) -> begin
 (
 
 let body = (desugar_term env t2)
@@ -1957,12 +1963,12 @@ end
 | FStar_Parser_AST.Match (e, branches) -> begin
 (
 
-let desugar_branch = (fun _65_1434 -> (match (_65_1434) with
+let desugar_branch = (fun _65_1440 -> (match (_65_1440) with
 | (pat, wopt, b) -> begin
 (
 
-let _65_1437 = (desugar_match_pat env pat)
-in (match (_65_1437) with
+let _65_1443 = (desugar_match_pat env pat)
+in (match (_65_1443) with
 | (env, pat) -> begin
 (
 
@@ -2005,23 +2011,23 @@ in ((_160_553), (annot), (None)))
 in FStar_Syntax_Syntax.Tm_ascribed (_160_554))
 in (FStar_All.pipe_left mk _160_555)))))
 end
-| FStar_Parser_AST.Record (_65_1451, []) -> begin
+| FStar_Parser_AST.Record (_65_1457, []) -> begin
 (Prims.raise (FStar_Syntax_Syntax.Error ((("Unexpected empty record"), (top.FStar_Parser_AST.range)))))
 end
 | FStar_Parser_AST.Record (eopt, fields) -> begin
 (
 
-let _65_1462 = (FStar_List.hd fields)
-in (match (_65_1462) with
-| (f, _65_1461) -> begin
+let _65_1468 = (FStar_List.hd fields)
+in (match (_65_1468) with
+| (f, _65_1467) -> begin
 (
 
-let _65_1466 = (FStar_Parser_Env.fail_or env (FStar_Parser_Env.try_lookup_record_by_field_name env) f)
-in (match (_65_1466) with
-| (record, _65_1465) -> begin
+let _65_1472 = (FStar_Parser_Env.fail_or env (FStar_Parser_Env.try_lookup_record_by_field_name env) f)
+in (match (_65_1472) with
+| (record, _65_1471) -> begin
 (
 
-let fields' = (FStar_All.pipe_right fields (FStar_List.map (fun _65_1469 -> (match (_65_1469) with
+let fields' = (FStar_All.pipe_right fields (FStar_List.map (fun _65_1475 -> (match (_65_1475) with
 | (f, e) -> begin
 (let _160_557 = (FStar_Syntax_Util.mk_field_projector_name_from_ident record.FStar_Parser_Env.constrname f.FStar_Ident.ident)
 in ((_160_557), (e)))
@@ -2030,12 +2036,12 @@ in (
 
 let get_field = (fun xopt f -> (
 
-let found = (FStar_All.pipe_right fields' (FStar_Util.find_opt (fun _65_1477 -> (match (_65_1477) with
-| (g, _65_1476) -> begin
+let found = (FStar_All.pipe_right fields' (FStar_Util.find_opt (fun _65_1483 -> (match (_65_1483) with
+| (g, _65_1482) -> begin
 (FStar_Ident.lid_equals f g)
 end))))
 in (match (found) with
-| Some (_65_1480, e) -> begin
+| Some (_65_1486, e) -> begin
 ((f), (e))
 end
 | None -> begin
@@ -2054,8 +2060,8 @@ in (
 
 let recterm = (match (eopt) with
 | None -> begin
-(let _160_570 = (let _160_569 = (FStar_All.pipe_right record.FStar_Parser_Env.fields (FStar_List.map (fun _65_1492 -> (match (_65_1492) with
-| (f, _65_1491) -> begin
+(let _160_570 = (let _160_569 = (FStar_All.pipe_right record.FStar_Parser_Env.fields (FStar_List.map (fun _65_1498 -> (match (_65_1498) with
+| (f, _65_1497) -> begin
 (let _160_568 = (let _160_567 = (get_field None f)
 in (FStar_All.pipe_left Prims.snd _160_567))
 in ((_160_568), (FStar_Parser_AST.Nothing)))
@@ -2074,8 +2080,8 @@ in FStar_Parser_AST.Var (_160_571))
 in (FStar_Parser_AST.mk_term _160_572 x.FStar_Ident.idRange FStar_Parser_AST.Expr))
 in (
 
-let record = (let _160_575 = (let _160_574 = (FStar_All.pipe_right record.FStar_Parser_Env.fields (FStar_List.map (fun _65_1500 -> (match (_65_1500) with
-| (f, _65_1499) -> begin
+let record = (let _160_575 = (let _160_574 = (FStar_All.pipe_right record.FStar_Parser_Env.fields (FStar_List.map (fun _65_1506 -> (match (_65_1506) with
+| (f, _65_1505) -> begin
 (get_field (Some (xterm)) f)
 end))))
 in ((None), (_160_574)))
@@ -2089,7 +2095,7 @@ in (
 
 let e = (desugar_term env recterm)
 in (match (e.FStar_Syntax_Syntax.n) with
-| FStar_Syntax_Syntax.Tm_meta ({FStar_Syntax_Syntax.n = FStar_Syntax_Syntax.Tm_app ({FStar_Syntax_Syntax.n = FStar_Syntax_Syntax.Tm_fvar (fv); FStar_Syntax_Syntax.tk = _65_1516; FStar_Syntax_Syntax.pos = _65_1514; FStar_Syntax_Syntax.vars = _65_1512}, args); FStar_Syntax_Syntax.tk = _65_1510; FStar_Syntax_Syntax.pos = _65_1508; FStar_Syntax_Syntax.vars = _65_1506}, FStar_Syntax_Syntax.Meta_desugared (FStar_Syntax_Syntax.Data_app)) -> begin
+| FStar_Syntax_Syntax.Tm_meta ({FStar_Syntax_Syntax.n = FStar_Syntax_Syntax.Tm_app ({FStar_Syntax_Syntax.n = FStar_Syntax_Syntax.Tm_fvar (fv); FStar_Syntax_Syntax.tk = _65_1522; FStar_Syntax_Syntax.pos = _65_1520; FStar_Syntax_Syntax.vars = _65_1518}, args); FStar_Syntax_Syntax.tk = _65_1516; FStar_Syntax_Syntax.pos = _65_1514; FStar_Syntax_Syntax.vars = _65_1512}, FStar_Syntax_Syntax.Meta_desugared (FStar_Syntax_Syntax.Data_app)) -> begin
 (
 
 let e = (let _160_582 = (let _160_581 = (let _160_580 = (let _160_579 = (let _160_578 = (let _160_577 = (let _160_576 = (FStar_All.pipe_right record.FStar_Parser_Env.fields (FStar_List.map Prims.fst))
@@ -2102,7 +2108,7 @@ in FStar_Syntax_Syntax.Tm_app (_160_581))
 in (FStar_All.pipe_left mk _160_582))
 in (FStar_All.pipe_left mk (FStar_Syntax_Syntax.Tm_meta (((e), (FStar_Syntax_Syntax.Meta_desugared (FStar_Syntax_Syntax.Data_app)))))))
 end
-| _65_1530 -> begin
+| _65_1536 -> begin
 e
 end))))))
 end))
@@ -2111,8 +2117,8 @@ end
 | FStar_Parser_AST.Project (e, f) -> begin
 (
 
-let _65_1537 = (FStar_Parser_Env.fail_or env (FStar_Parser_Env.try_lookup_projector_by_field_name env) f)
-in (match (_65_1537) with
+let _65_1543 = (FStar_Parser_Env.fail_or env (FStar_Parser_Env.try_lookup_projector_by_field_name env) f)
+in (match (_65_1543) with
 | (fieldname, is_rec) -> begin
 (
 
@@ -2138,22 +2144,22 @@ end
 | (FStar_Parser_AST.NamedTyp (_, e)) | (FStar_Parser_AST.Paren (e)) -> begin
 (desugar_term env e)
 end
-| _65_1548 when (top.FStar_Parser_AST.level = FStar_Parser_AST.Formula) -> begin
+| _65_1554 when (top.FStar_Parser_AST.level = FStar_Parser_AST.Formula) -> begin
 (desugar_formula env top)
 end
-| _65_1550 -> begin
+| _65_1556 -> begin
 (FStar_Parser_AST.error "Unexpected term" top top.FStar_Parser_AST.range)
 end
-| FStar_Parser_AST.Let (_65_1552, _65_1554, _65_1556) -> begin
+| FStar_Parser_AST.Let (_65_1558, _65_1560, _65_1562) -> begin
 (FStar_All.failwith "Not implemented yet")
 end
-| FStar_Parser_AST.QForall (_65_1560, _65_1562, _65_1564) -> begin
+| FStar_Parser_AST.QForall (_65_1566, _65_1568, _65_1570) -> begin
 (FStar_All.failwith "Not implemented yet")
 end
-| FStar_Parser_AST.QExists (_65_1568, _65_1570, _65_1572) -> begin
+| FStar_Parser_AST.QExists (_65_1574, _65_1576, _65_1578) -> begin
 (FStar_All.failwith "Not implemented yet")
 end))))
-and desugar_args : FStar_Parser_Env.env  ->  (FStar_Parser_AST.term * FStar_Parser_AST.imp) Prims.list  ->  (FStar_Syntax_Syntax.term * FStar_Syntax_Syntax.arg_qualifier Prims.option) Prims.list = (fun env args -> (FStar_All.pipe_right args (FStar_List.map (fun _65_1579 -> (match (_65_1579) with
+and desugar_args : FStar_Parser_Env.env  ->  (FStar_Parser_AST.term * FStar_Parser_AST.imp) Prims.list  ->  (FStar_Syntax_Syntax.term * FStar_Syntax_Syntax.arg_qualifier Prims.option) Prims.list = (fun env args -> (FStar_All.pipe_right args (FStar_List.map (fun _65_1585 -> (match (_65_1585) with
 | (a, imp) -> begin
 (let _160_591 = (desugar_term env a)
 in (arg_withimp_e imp _160_591))
@@ -2163,40 +2169,40 @@ and desugar_comp : FStar_Range.range  ->  Prims.bool  ->  FStar_Parser_Env.env  
 let fail = (fun msg -> (Prims.raise (FStar_Syntax_Syntax.Error (((msg), (r))))))
 in (
 
-let is_requires = (fun _65_1591 -> (match (_65_1591) with
-| (t, _65_1590) -> begin
+let is_requires = (fun _65_1597 -> (match (_65_1597) with
+| (t, _65_1596) -> begin
 (match ((let _160_599 = (unparen t)
 in _160_599.FStar_Parser_AST.tm)) with
-| FStar_Parser_AST.Requires (_65_1593) -> begin
+| FStar_Parser_AST.Requires (_65_1599) -> begin
 true
 end
-| _65_1596 -> begin
+| _65_1602 -> begin
 false
 end)
 end))
 in (
 
-let is_ensures = (fun _65_1601 -> (match (_65_1601) with
-| (t, _65_1600) -> begin
+let is_ensures = (fun _65_1607 -> (match (_65_1607) with
+| (t, _65_1606) -> begin
 (match ((let _160_602 = (unparen t)
 in _160_602.FStar_Parser_AST.tm)) with
-| FStar_Parser_AST.Ensures (_65_1603) -> begin
+| FStar_Parser_AST.Ensures (_65_1609) -> begin
 true
 end
-| _65_1606 -> begin
+| _65_1612 -> begin
 false
 end)
 end))
 in (
 
-let is_app = (fun head _65_1612 -> (match (_65_1612) with
-| (t, _65_1611) -> begin
+let is_app = (fun head _65_1618 -> (match (_65_1618) with
+| (t, _65_1617) -> begin
 (match ((let _160_607 = (unparen t)
 in _160_607.FStar_Parser_AST.tm)) with
-| FStar_Parser_AST.App ({FStar_Parser_AST.tm = FStar_Parser_AST.Var (d); FStar_Parser_AST.range = _65_1616; FStar_Parser_AST.level = _65_1614}, _65_1621, _65_1623) -> begin
+| FStar_Parser_AST.App ({FStar_Parser_AST.tm = FStar_Parser_AST.Var (d); FStar_Parser_AST.range = _65_1622; FStar_Parser_AST.level = _65_1620}, _65_1627, _65_1629) -> begin
 (d.FStar_Ident.ident.FStar_Ident.idText = head)
 end
-| _65_1627 -> begin
+| _65_1633 -> begin
 false
 end)
 end))
@@ -2207,8 +2213,8 @@ in (
 
 let pre_process_comp_typ = (fun t -> (
 
-let _65_1633 = (head_and_args t)
-in (match (_65_1633) with
+let _65_1639 = (head_and_args t)
+in (match (_65_1639) with
 | (head, args) -> begin
 (match (head.FStar_Parser_AST.tm) with
 | FStar_Parser_AST.Name (lemma) when (lemma.FStar_Ident.ident.FStar_Ident.idText = "Lemma") -> begin
@@ -2262,10 +2268,10 @@ end
 | FStar_Parser_AST.Name (l) when ((((l.FStar_Ident.ident.FStar_Ident.idText = "Type") || (l.FStar_Ident.ident.FStar_Ident.idText = "Type0")) || (l.FStar_Ident.ident.FStar_Ident.idText = "Effect")) && default_ok) -> begin
 (((FStar_Ident.set_lid_range FStar_Syntax_Const.effect_Tot_lid head.FStar_Parser_AST.range)), ((((t), (FStar_Parser_AST.Nothing)))::[]))
 end
-| _65_1664 when default_ok -> begin
+| _65_1670 when default_ok -> begin
 (((FStar_Ident.set_lid_range env.FStar_Parser_Env.default_result_effect head.FStar_Parser_AST.range)), ((((t), (FStar_Parser_AST.Nothing)))::[]))
 end
-| _65_1666 -> begin
+| _65_1672 -> begin
 (let _160_615 = (let _160_614 = (FStar_Parser_AST.term_to_string t)
 in (FStar_Util.format1 "%s is not an effect" _160_614))
 in (fail _160_615))
@@ -2273,12 +2279,12 @@ end)
 end)))
 in (
 
-let _65_1669 = (pre_process_comp_typ t)
-in (match (_65_1669) with
+let _65_1675 = (pre_process_comp_typ t)
+in (match (_65_1675) with
 | (eff, args) -> begin
 (
 
-let _65_1670 = if ((FStar_List.length args) = (Prims.parse_int "0")) then begin
+let _65_1676 = if ((FStar_List.length args) = (Prims.parse_int "0")) then begin
 (let _160_617 = (let _160_616 = (FStar_Syntax_Print.lid_to_string eff)
 in (FStar_Util.format1 "Not enough args to effect %s" _160_616))
 in (fail _160_617))
@@ -2287,10 +2293,10 @@ end else begin
 end
 in (
 
-let _65_1674 = (let _160_619 = (FStar_List.hd args)
+let _65_1680 = (let _160_619 = (FStar_List.hd args)
 in (let _160_618 = (FStar_List.tl args)
 in ((_160_619), (_160_618))))
-in (match (_65_1674) with
+in (match (_65_1680) with
 | (result_arg, rest) -> begin
 (
 
@@ -2300,27 +2306,27 @@ in (
 let rest = (desugar_args env rest)
 in (
 
-let _65_1699 = (FStar_All.pipe_right rest (FStar_List.partition (fun _65_1680 -> (match (_65_1680) with
-| (t, _65_1679) -> begin
+let _65_1705 = (FStar_All.pipe_right rest (FStar_List.partition (fun _65_1686 -> (match (_65_1686) with
+| (t, _65_1685) -> begin
 (match (t.FStar_Syntax_Syntax.n) with
-| FStar_Syntax_Syntax.Tm_app ({FStar_Syntax_Syntax.n = FStar_Syntax_Syntax.Tm_fvar (fv); FStar_Syntax_Syntax.tk = _65_1686; FStar_Syntax_Syntax.pos = _65_1684; FStar_Syntax_Syntax.vars = _65_1682}, (_65_1691)::[]) -> begin
+| FStar_Syntax_Syntax.Tm_app ({FStar_Syntax_Syntax.n = FStar_Syntax_Syntax.Tm_fvar (fv); FStar_Syntax_Syntax.tk = _65_1692; FStar_Syntax_Syntax.pos = _65_1690; FStar_Syntax_Syntax.vars = _65_1688}, (_65_1697)::[]) -> begin
 (FStar_Syntax_Syntax.fv_eq_lid fv FStar_Syntax_Const.decreases_lid)
 end
-| _65_1696 -> begin
+| _65_1702 -> begin
 false
 end)
 end))))
-in (match (_65_1699) with
+in (match (_65_1705) with
 | (dec, rest) -> begin
 (
 
-let decreases_clause = (FStar_All.pipe_right dec (FStar_List.map (fun _65_1703 -> (match (_65_1703) with
-| (t, _65_1702) -> begin
+let decreases_clause = (FStar_All.pipe_right dec (FStar_List.map (fun _65_1709 -> (match (_65_1709) with
+| (t, _65_1708) -> begin
 (match (t.FStar_Syntax_Syntax.n) with
-| FStar_Syntax_Syntax.Tm_app (_65_1705, ((arg, _65_1708))::[]) -> begin
+| FStar_Syntax_Syntax.Tm_app (_65_1711, ((arg, _65_1714))::[]) -> begin
 FStar_Syntax_Syntax.DECREASES (arg)
 end
-| _65_1714 -> begin
+| _65_1720 -> begin
 (FStar_All.failwith "impos")
 end)
 end))))
@@ -2370,7 +2376,7 @@ let pattern = (let _160_622 = (FStar_Syntax_Syntax.fvar (FStar_Ident.set_lid_ran
 in (FStar_Syntax_Syntax.mk_Tm_uinst _160_622 ((FStar_Syntax_Syntax.U_zero)::[])))
 in (FStar_Syntax_Syntax.mk_Tm_app nil ((((pattern), (Some (FStar_Syntax_Syntax.imp_tag))))::[]) None pat.FStar_Syntax_Syntax.pos)))
 end
-| _65_1729 -> begin
+| _65_1735 -> begin
 pat
 end)
 in (let _160_626 = (let _160_625 = (let _160_624 = (let _160_623 = (FStar_Syntax_Syntax.mk (FStar_Syntax_Syntax.Tm_meta (((pat), (FStar_Syntax_Syntax.Meta_desugared (FStar_Syntax_Syntax.Meta_smt_pat))))) None pat.FStar_Syntax_Syntax.pos)
@@ -2379,7 +2385,7 @@ in (_160_624)::[])
 in (ens)::_160_625)
 in (req)::_160_626))
 end
-| _65_1732 -> begin
+| _65_1738 -> begin
 rest
 end)
 end else begin
@@ -2409,7 +2415,7 @@ end
 | "~" -> begin
 Some (FStar_Syntax_Const.not_lid)
 end
-| _65_1744 -> begin
+| _65_1750 -> begin
 None
 end))
 in (
@@ -2422,16 +2428,16 @@ in (
 
 let setpos = (fun t -> (
 
-let _65_1751 = t
-in {FStar_Syntax_Syntax.n = _65_1751.FStar_Syntax_Syntax.n; FStar_Syntax_Syntax.tk = _65_1751.FStar_Syntax_Syntax.tk; FStar_Syntax_Syntax.pos = f.FStar_Parser_AST.range; FStar_Syntax_Syntax.vars = _65_1751.FStar_Syntax_Syntax.vars}))
+let _65_1757 = t
+in {FStar_Syntax_Syntax.n = _65_1757.FStar_Syntax_Syntax.n; FStar_Syntax_Syntax.tk = _65_1757.FStar_Syntax_Syntax.tk; FStar_Syntax_Syntax.pos = f.FStar_Parser_AST.range; FStar_Syntax_Syntax.vars = _65_1757.FStar_Syntax_Syntax.vars}))
 in (
 
 let desugar_quant = (fun q b pats body -> (
 
 let tk = (desugar_binder env (
 
-let _65_1758 = b
-in {FStar_Parser_AST.b = _65_1758.FStar_Parser_AST.b; FStar_Parser_AST.brange = _65_1758.FStar_Parser_AST.brange; FStar_Parser_AST.blevel = FStar_Parser_AST.Formula; FStar_Parser_AST.aqual = _65_1758.FStar_Parser_AST.aqual}))
+let _65_1764 = b
+in {FStar_Parser_AST.b = _65_1764.FStar_Parser_AST.b; FStar_Parser_AST.brange = _65_1764.FStar_Parser_AST.brange; FStar_Parser_AST.blevel = FStar_Parser_AST.Formula; FStar_Parser_AST.aqual = _65_1764.FStar_Parser_AST.aqual}))
 in (
 
 let desugar_pats = (fun env pats -> (FStar_List.map (fun es -> (FStar_All.pipe_right es (FStar_List.map (fun e -> (let _160_661 = (desugar_term env e)
@@ -2440,15 +2446,15 @@ in (match (tk) with
 | (Some (a), k) -> begin
 (
 
-let _65_1772 = (FStar_Parser_Env.push_bv env a)
-in (match (_65_1772) with
+let _65_1778 = (FStar_Parser_Env.push_bv env a)
+in (match (_65_1778) with
 | (env, a) -> begin
 (
 
 let a = (
 
-let _65_1773 = a
-in {FStar_Syntax_Syntax.ppname = _65_1773.FStar_Syntax_Syntax.ppname; FStar_Syntax_Syntax.index = _65_1773.FStar_Syntax_Syntax.index; FStar_Syntax_Syntax.sort = k})
+let _65_1779 = a
+in {FStar_Syntax_Syntax.ppname = _65_1779.FStar_Syntax_Syntax.ppname; FStar_Syntax_Syntax.index = _65_1779.FStar_Syntax_Syntax.index; FStar_Syntax_Syntax.sort = k})
 in (
 
 let pats = (desugar_pats env pats)
@@ -2461,7 +2467,7 @@ let body = (match (pats) with
 | [] -> begin
 body
 end
-| _65_1780 -> begin
+| _65_1786 -> begin
 (mk (FStar_Syntax_Syntax.Tm_meta (((body), (FStar_Syntax_Syntax.Meta_pattern (pats))))))
 end)
 in (
@@ -2478,7 +2484,7 @@ in FStar_Syntax_Syntax.Tm_app (_160_668))
 in (FStar_All.pipe_left mk _160_669)))))))
 end))
 end
-| _65_1784 -> begin
+| _65_1790 -> begin
 (FStar_All.failwith "impossible")
 end))))
 in (
@@ -2496,7 +2502,7 @@ in (FStar_Parser_AST.mk_term _160_684 _160_683 FStar_Parser_AST.Formula)))
 in (let _160_685 = (q (((b)::[]), ([]), (body)))
 in (FStar_Parser_AST.mk_term _160_685 f.FStar_Parser_AST.range FStar_Parser_AST.Formula))))
 end
-| _65_1798 -> begin
+| _65_1804 -> begin
 (FStar_All.failwith "impossible")
 end))
 in (match ((let _160_686 = (unparen f)
@@ -2533,40 +2539,40 @@ end
 | FStar_Parser_AST.Paren (f) -> begin
 (desugar_formula env f)
 end
-| _65_1856 -> begin
+| _65_1862 -> begin
 (desugar_term env f)
 end))))))))
 and typars_of_binders : FStar_Parser_Env.env  ->  FStar_Parser_AST.binder Prims.list  ->  (FStar_Parser_Env.env * (FStar_Syntax_Syntax.bv * FStar_Syntax_Syntax.arg_qualifier Prims.option) Prims.list) = (fun env bs -> (
 
-let _65_1880 = (FStar_List.fold_left (fun _65_1861 b -> (match (_65_1861) with
+let _65_1886 = (FStar_List.fold_left (fun _65_1867 b -> (match (_65_1867) with
 | (env, out) -> begin
 (
 
 let tk = (desugar_binder env (
 
-let _65_1863 = b
-in {FStar_Parser_AST.b = _65_1863.FStar_Parser_AST.b; FStar_Parser_AST.brange = _65_1863.FStar_Parser_AST.brange; FStar_Parser_AST.blevel = FStar_Parser_AST.Formula; FStar_Parser_AST.aqual = _65_1863.FStar_Parser_AST.aqual}))
+let _65_1869 = b
+in {FStar_Parser_AST.b = _65_1869.FStar_Parser_AST.b; FStar_Parser_AST.brange = _65_1869.FStar_Parser_AST.brange; FStar_Parser_AST.blevel = FStar_Parser_AST.Formula; FStar_Parser_AST.aqual = _65_1869.FStar_Parser_AST.aqual}))
 in (match (tk) with
 | (Some (a), k) -> begin
 (
 
-let _65_1872 = (FStar_Parser_Env.push_bv env a)
-in (match (_65_1872) with
+let _65_1878 = (FStar_Parser_Env.push_bv env a)
+in (match (_65_1878) with
 | (env, a) -> begin
 (
 
 let a = (
 
-let _65_1873 = a
-in {FStar_Syntax_Syntax.ppname = _65_1873.FStar_Syntax_Syntax.ppname; FStar_Syntax_Syntax.index = _65_1873.FStar_Syntax_Syntax.index; FStar_Syntax_Syntax.sort = k})
+let _65_1879 = a
+in {FStar_Syntax_Syntax.ppname = _65_1879.FStar_Syntax_Syntax.ppname; FStar_Syntax_Syntax.index = _65_1879.FStar_Syntax_Syntax.index; FStar_Syntax_Syntax.sort = k})
 in ((env), ((((a), ((trans_aqual b.FStar_Parser_AST.aqual))))::out)))
 end))
 end
-| _65_1877 -> begin
+| _65_1883 -> begin
 (Prims.raise (FStar_Syntax_Syntax.Error ((("Unexpected binder"), (b.FStar_Parser_AST.brange)))))
 end))
 end)) ((env), ([])) bs)
-in (match (_65_1880) with
+in (match (_65_1886) with
 | (env, tpars) -> begin
 ((env), ((FStar_List.rev tpars)))
 end)))
@@ -2594,7 +2600,7 @@ let quals = (FStar_All.pipe_right quals (FStar_List.filter (fun _65_11 -> (match
 | (FStar_Syntax_Syntax.Abstract) | (FStar_Syntax_Syntax.Private) -> begin
 true
 end
-| _65_1905 -> begin
+| _65_1911 -> begin
 false
 end))))
 in (
@@ -2614,13 +2620,13 @@ in (
 let p = (FStar_Ident.range_of_lid t)
 in (
 
-let _65_1913 = (FStar_Syntax_Util.args_of_binders binders)
-in (match (_65_1913) with
+let _65_1919 = (FStar_Syntax_Util.args_of_binders binders)
+in (match (_65_1919) with
 | (binders, args) -> begin
 (
 
-let imp_binders = (FStar_All.pipe_right binders (FStar_List.map (fun _65_1917 -> (match (_65_1917) with
-| (x, _65_1916) -> begin
+let imp_binders = (FStar_All.pipe_right binders (FStar_List.map (fun _65_1923 -> (match (_65_1923) with
+| (x, _65_1922) -> begin
 ((x), (Some (FStar_Syntax_Syntax.imp_tag)))
 end))))
 in (
@@ -2657,50 +2663,50 @@ in (
 let projectee = (fun ptyp -> (FStar_Syntax_Syntax.gen_bv "projectee" (Some (p)) ptyp))
 in (
 
-let tps = (FStar_List.map2 (fun _65_1941 _65_1945 -> (match (((_65_1941), (_65_1945))) with
-| ((_65_1939, imp), (x, _65_1944)) -> begin
+let tps = (FStar_List.map2 (fun _65_1947 _65_1951 -> (match (((_65_1947), (_65_1951))) with
+| ((_65_1945, imp), (x, _65_1950)) -> begin
 ((x), (imp))
 end)) inductive_tps imp_tps)
 in (
 
-let _65_2046 = (
+let _65_2052 = (
 
-let _65_1949 = (FStar_Syntax_Util.head_and_args t)
-in (match (_65_1949) with
+let _65_1955 = (FStar_Syntax_Util.head_and_args t)
+in (match (_65_1955) with
 | (head, args0) -> begin
 (
 
 let args = (
 
 let rec arguments = (fun tps args -> (match (((tps), (args))) with
-| ([], _65_1955) -> begin
+| ([], _65_1961) -> begin
 args
 end
-| (_65_1958, []) -> begin
+| (_65_1964, []) -> begin
 (Prims.raise (FStar_Syntax_Syntax.Error ((("Not enough arguments to type"), ((FStar_Ident.range_of_lid lid))))))
 end
-| (((_65_1963, Some (FStar_Syntax_Syntax.Implicit (_65_1965))))::tps', ((_65_1972, Some (FStar_Syntax_Syntax.Implicit (_65_1974))))::args') -> begin
+| (((_65_1969, Some (FStar_Syntax_Syntax.Implicit (_65_1971))))::tps', ((_65_1978, Some (FStar_Syntax_Syntax.Implicit (_65_1980))))::args') -> begin
 (arguments tps' args')
 end
-| (((_65_1982, Some (FStar_Syntax_Syntax.Implicit (_65_1984))))::tps', ((_65_1992, _65_1994))::_65_1990) -> begin
+| (((_65_1988, Some (FStar_Syntax_Syntax.Implicit (_65_1990))))::tps', ((_65_1998, _65_2000))::_65_1996) -> begin
 (arguments tps' args)
 end
-| (((_65_2001, _65_2003))::_65_1999, ((a, Some (FStar_Syntax_Syntax.Implicit (_65_2010))))::_65_2007) -> begin
+| (((_65_2007, _65_2009))::_65_2005, ((a, Some (FStar_Syntax_Syntax.Implicit (_65_2016))))::_65_2013) -> begin
 (Prims.raise (FStar_Syntax_Syntax.Error ((("Unexpected implicit annotation on argument"), (a.FStar_Syntax_Syntax.pos)))))
 end
-| (((_65_2018, _65_2020))::tps', ((_65_2025, _65_2027))::args') -> begin
+| (((_65_2024, _65_2026))::tps', ((_65_2031, _65_2033))::args') -> begin
 (arguments tps' args')
 end))
 in (arguments inductive_tps args0))
 in (
 
-let indices = (FStar_All.pipe_right args (FStar_List.map (fun _65_2032 -> (let _160_760 = (FStar_Syntax_Syntax.new_bv (Some (p)) FStar_Syntax_Syntax.tun)
+let indices = (FStar_All.pipe_right args (FStar_List.map (fun _65_2038 -> (let _160_760 = (FStar_Syntax_Syntax.new_bv (Some (p)) FStar_Syntax_Syntax.tun)
 in (FStar_All.pipe_right _160_760 FStar_Syntax_Syntax.mk_binder)))))
 in (
 
 let arg_typ = (let _160_765 = (let _160_761 = (FStar_Syntax_Syntax.lid_as_fv tc FStar_Syntax_Syntax.Delta_constant None)
 in (FStar_Syntax_Syntax.fv_to_tm _160_761))
-in (let _160_764 = (FStar_All.pipe_right (FStar_List.append tps indices) (FStar_List.map (fun _65_2037 -> (match (_65_2037) with
+in (let _160_764 = (FStar_All.pipe_right (FStar_List.append tps indices) (FStar_List.map (fun _65_2043 -> (match (_65_2043) with
 | (x, imp) -> begin
 (let _160_763 = (FStar_Syntax_Syntax.bv_to_name x)
 in ((_160_763), (imp)))
@@ -2720,7 +2726,7 @@ in (
 let x = (FStar_Syntax_Syntax.new_bv (Some (p)) arg_typ)
 in (let _160_774 = (
 
-let _65_2041 = (projectee arg_typ)
+let _65_2047 = (projectee arg_typ)
 in (let _160_773 = (let _160_772 = (let _160_771 = (let _160_770 = (FStar_Syntax_Syntax.fvar (FStar_Ident.set_lid_range disc_name p) FStar_Syntax_Syntax.Delta_equational None)
 in (let _160_769 = (let _160_768 = (let _160_767 = (FStar_Syntax_Syntax.bv_to_name x)
 in (FStar_All.pipe_left FStar_Syntax_Syntax.as_arg _160_767))
@@ -2728,20 +2734,20 @@ in (_160_768)::[])
 in (FStar_Syntax_Syntax.mk_Tm_app _160_770 _160_769 None p)))
 in (FStar_Syntax_Util.b2t _160_771))
 in (FStar_Syntax_Util.refine x _160_772))
-in {FStar_Syntax_Syntax.ppname = _65_2041.FStar_Syntax_Syntax.ppname; FStar_Syntax_Syntax.index = _65_2041.FStar_Syntax_Syntax.index; FStar_Syntax_Syntax.sort = _160_773}))
+in {FStar_Syntax_Syntax.ppname = _65_2047.FStar_Syntax_Syntax.ppname; FStar_Syntax_Syntax.index = _65_2047.FStar_Syntax_Syntax.index; FStar_Syntax_Syntax.sort = _160_773}))
 in (FStar_Syntax_Syntax.mk_binder _160_774))))
 end
 in ((arg_binder), (indices))))))
 end))
-in (match (_65_2046) with
+in (match (_65_2052) with
 | (arg_binder, indices) -> begin
 (
 
 let arg_exp = (FStar_Syntax_Syntax.bv_to_name (Prims.fst arg_binder))
 in (
 
-let imp_binders = (let _160_776 = (FStar_All.pipe_right indices (FStar_List.map (fun _65_2051 -> (match (_65_2051) with
-| (x, _65_2050) -> begin
+let imp_binders = (let _160_776 = (FStar_All.pipe_right indices (FStar_List.map (fun _65_2057 -> (match (_65_2057) with
+| (x, _65_2056) -> begin
 ((x), (Some (FStar_Syntax_Syntax.imp_tag)))
 end))))
 in (FStar_List.append imp_tps _160_776))
@@ -2753,13 +2759,13 @@ in (
 let arg = (FStar_Syntax_Util.arg_of_non_null_binder arg_binder)
 in (
 
-let subst = (FStar_All.pipe_right fields (FStar_List.mapi (fun i _65_2059 -> (match (_65_2059) with
-| (a, _65_2058) -> begin
+let subst = (FStar_All.pipe_right fields (FStar_List.mapi (fun i _65_2065 -> (match (_65_2065) with
+| (a, _65_2064) -> begin
 (
 
-let _65_2063 = (FStar_Syntax_Util.mk_field_projector_name lid a i)
-in (match (_65_2063) with
-| (field_name, _65_2062) -> begin
+let _65_2069 = (FStar_Syntax_Util.mk_field_projector_name lid a i)
+in (match (_65_2069) with
+| (field_name, _65_2068) -> begin
 (
 
 let proj = (let _160_780 = (let _160_779 = (FStar_Syntax_Syntax.lid_as_fv field_name FStar_Syntax_Syntax.Delta_equational None)
@@ -2774,13 +2780,13 @@ let ntps = (FStar_List.length tps)
 in (
 
 let all_params = (FStar_List.append imp_tps fields)
-in (let _160_819 = (FStar_All.pipe_right fields (FStar_List.mapi (fun i _65_2072 -> (match (_65_2072) with
-| (x, _65_2071) -> begin
+in (let _160_819 = (FStar_All.pipe_right fields (FStar_List.mapi (fun i _65_2078 -> (match (_65_2078) with
+| (x, _65_2077) -> begin
 (
 
-let _65_2076 = (FStar_Syntax_Util.mk_field_projector_name lid x i)
-in (match (_65_2076) with
-| (field_name, _65_2075) -> begin
+let _65_2082 = (FStar_Syntax_Util.mk_field_projector_name lid x i)
+in (match (_65_2082) with
+| (field_name, _65_2081) -> begin
 (
 
 let t = (let _160_784 = (let _160_783 = (FStar_Syntax_Subst.subst subst x.FStar_Syntax_Syntax.sort)
@@ -2802,7 +2808,7 @@ let quals = (fun q -> if only_decl then begin
 | FStar_Syntax_Syntax.Abstract -> begin
 false
 end
-| _65_2085 -> begin
+| _65_2091 -> begin
 true
 end)) q)
 in (FStar_Syntax_Syntax.Assumption)::_160_791)
@@ -2817,7 +2823,7 @@ let iquals = (FStar_All.pipe_right iquals (FStar_List.filter (fun _65_13 -> (mat
 | (FStar_Syntax_Syntax.Abstract) | (FStar_Syntax_Syntax.Private) -> begin
 true
 end
-| _65_2090 -> begin
+| _65_2096 -> begin
 false
 end))))
 in (quals ((FStar_Syntax_Syntax.Projector (((lid), (x.FStar_Syntax_Syntax.ppname))))::iquals)))
@@ -2832,7 +2838,7 @@ end else begin
 let projection = (FStar_Syntax_Syntax.gen_bv x.FStar_Syntax_Syntax.ppname.FStar_Ident.idText None FStar_Syntax_Syntax.tun)
 in (
 
-let arg_pats = (FStar_All.pipe_right all_params (FStar_List.mapi (fun j _65_2098 -> (match (_65_2098) with
+let arg_pats = (FStar_All.pipe_right all_params (FStar_List.mapi (fun j _65_2104 -> (match (_65_2104) with
 | (x, imp) -> begin
 (
 
@@ -2904,17 +2910,17 @@ in (FStar_All.pipe_right _160_819 FStar_List.flatten)))))))))
 end)))))))
 
 
-let mk_data_projectors : FStar_Syntax_Syntax.qualifier Prims.list  ->  FStar_Parser_Env.env  ->  (FStar_Syntax_Syntax.binders * FStar_Syntax_Syntax.sigelt)  ->  FStar_Syntax_Syntax.sigelt Prims.list = (fun iquals env _65_2112 -> (match (_65_2112) with
+let mk_data_projectors : FStar_Syntax_Syntax.qualifier Prims.list  ->  FStar_Parser_Env.env  ->  (FStar_Syntax_Syntax.binders * FStar_Syntax_Syntax.sigelt)  ->  FStar_Syntax_Syntax.sigelt Prims.list = (fun iquals env _65_2118 -> (match (_65_2118) with
 | (inductive_tps, se) -> begin
 (match (se) with
-| FStar_Syntax_Syntax.Sig_datacon (lid, _65_2115, t, l, n, quals, _65_2121, _65_2123) when (not ((FStar_Ident.lid_equals lid FStar_Syntax_Const.lexcons_lid))) -> begin
+| FStar_Syntax_Syntax.Sig_datacon (lid, _65_2121, t, l, n, quals, _65_2127, _65_2129) when (not ((FStar_Ident.lid_equals lid FStar_Syntax_Const.lexcons_lid))) -> begin
 (
 
 let refine_domain = if (FStar_All.pipe_right quals (FStar_Util.for_some (fun _65_14 -> (match (_65_14) with
-| FStar_Syntax_Syntax.RecordConstructor (_65_2128) -> begin
+| FStar_Syntax_Syntax.RecordConstructor (_65_2134) -> begin
 true
 end
-| _65_2131 -> begin
+| _65_2137 -> begin
 false
 end)))) then begin
 false
@@ -2923,27 +2929,27 @@ end else begin
 | Some (l) -> begin
 ((FStar_List.length l) > (Prims.parse_int "1"))
 end
-| _65_2135 -> begin
+| _65_2141 -> begin
 true
 end)
 end
 in (
 
-let _65_2139 = (FStar_Syntax_Util.arrow_formals t)
-in (match (_65_2139) with
+let _65_2145 = (FStar_Syntax_Util.arrow_formals t)
+in (match (_65_2145) with
 | (formals, cod) -> begin
 (match (formals) with
 | [] -> begin
 []
 end
-| _65_2142 -> begin
+| _65_2148 -> begin
 (
 
 let fv_qual = (match ((FStar_Util.find_map quals (fun _65_15 -> (match (_65_15) with
 | FStar_Syntax_Syntax.RecordConstructor (fns) -> begin
 Some (FStar_Syntax_Syntax.Record_ctor (((lid), (fns))))
 end
-| _65_2147 -> begin
+| _65_2153 -> begin
 None
 end)))) with
 | None -> begin
@@ -2961,15 +2967,15 @@ iquals
 end
 in (
 
-let _65_2155 = (FStar_Util.first_N n formals)
-in (match (_65_2155) with
+let _65_2161 = (FStar_Util.first_N n formals)
+in (match (_65_2161) with
 | (tps, rest) -> begin
 (mk_indexed_projectors iquals fv_qual refine_domain env l lid inductive_tps tps rest cod)
 end))))
 end)
 end)))
 end
-| _65_2157 -> begin
+| _65_2163 -> begin
 []
 end)
 end))
@@ -3028,7 +3034,7 @@ let imp_of_aqual = (fun b -> (match (b.FStar_Parser_AST.aqual) with
 | Some (FStar_Parser_AST.Implicit) -> begin
 FStar_Parser_AST.Hash
 end
-| _65_2232 -> begin
+| _65_2238 -> begin
 FStar_Parser_AST.Nothing
 end))
 in (FStar_List.fold_left (fun out b -> (let _160_876 = (let _160_875 = (let _160_874 = (binder_to_term b)
@@ -3044,8 +3050,8 @@ let tycon_record_as_variant = (fun _65_17 -> (match (_65_17) with
 let constrName = (FStar_Ident.mk_ident (((Prims.strcat "Mk" id.FStar_Ident.idText)), (id.FStar_Ident.idRange)))
 in (
 
-let mfields = (FStar_List.map (fun _65_2247 -> (match (_65_2247) with
-| (x, t, _65_2246) -> begin
+let mfields = (FStar_List.map (fun _65_2253 -> (match (_65_2253) with
+| (x, t, _65_2252) -> begin
 (FStar_Parser_AST.mk_binder (FStar_Parser_AST.Annotated ((((FStar_Syntax_Util.mangle_field_name x)), (t)))) x.FStar_Ident.idRange FStar_Parser_AST.Expr None)
 end)) fields)
 in (
@@ -3057,13 +3063,13 @@ in (apply_binders _160_882 parms))
 in (
 
 let constrTyp = (FStar_Parser_AST.mk_term (FStar_Parser_AST.Product (((mfields), ((with_constructor_effect result))))) id.FStar_Ident.idRange FStar_Parser_AST.Type)
-in (let _160_884 = (FStar_All.pipe_right fields (FStar_List.map (fun _65_2256 -> (match (_65_2256) with
-| (x, _65_2253, _65_2255) -> begin
+in (let _160_884 = (FStar_All.pipe_right fields (FStar_List.map (fun _65_2262 -> (match (_65_2262) with
+| (x, _65_2259, _65_2261) -> begin
 (FStar_Parser_Env.qualify env x)
 end))))
 in ((FStar_Parser_AST.TyconVariant (((id), (parms), (kopt), ((((constrName), (Some (constrTyp)), (None), (false)))::[])))), (_160_884)))))))
 end
-| _65_2258 -> begin
+| _65_2264 -> begin
 (FStar_All.failwith "impossible")
 end))
 in (
@@ -3072,8 +3078,8 @@ let desugar_abstract_tc = (fun quals _env mutuals _65_18 -> (match (_65_18) with
 | FStar_Parser_AST.TyconAbstract (id, binders, kopt) -> begin
 (
 
-let _65_2272 = (typars_of_binders _env binders)
-in (match (_65_2272) with
+let _65_2278 = (typars_of_binders _env binders)
+in (match (_65_2278) with
 | (_env', typars) -> begin
 (
 
@@ -3111,24 +3117,24 @@ let _env2 = (FStar_Parser_Env.push_top_level_rec_binding _env' id FStar_Syntax_S
 in ((_env), (_env2), (se), (tconstr))))))))))
 end))
 end
-| _65_2285 -> begin
+| _65_2291 -> begin
 (FStar_All.failwith "Unexpected tycon")
 end))
 in (
 
 let push_tparams = (fun env bs -> (
 
-let _65_2300 = (FStar_List.fold_left (fun _65_2291 _65_2294 -> (match (((_65_2291), (_65_2294))) with
+let _65_2306 = (FStar_List.fold_left (fun _65_2297 _65_2300 -> (match (((_65_2297), (_65_2300))) with
 | ((env, tps), (x, imp)) -> begin
 (
 
-let _65_2297 = (FStar_Parser_Env.push_bv env x.FStar_Syntax_Syntax.ppname)
-in (match (_65_2297) with
+let _65_2303 = (FStar_Parser_Env.push_bv env x.FStar_Syntax_Syntax.ppname)
+in (match (_65_2303) with
 | (env, y) -> begin
 ((env), ((((y), (imp)))::tps))
 end))
 end)) ((env), ([])) bs)
-in (match (_65_2300) with
+in (match (_65_2306) with
 | (env, bs) -> begin
 ((env), ((FStar_List.rev bs)))
 end)))
@@ -3141,7 +3147,7 @@ let kopt = (match (kopt) with
 (let _160_902 = (tm_type_z id.FStar_Ident.idRange)
 in Some (_160_902))
 end
-| _65_2309 -> begin
+| _65_2315 -> begin
 kopt
 end)
 in (
@@ -3149,13 +3155,13 @@ in (
 let tc = FStar_Parser_AST.TyconAbstract (((id), (bs), (kopt)))
 in (
 
-let _65_2319 = (desugar_abstract_tc quals env [] tc)
-in (match (_65_2319) with
-| (_65_2313, _65_2315, se, _65_2318) -> begin
+let _65_2325 = (desugar_abstract_tc quals env [] tc)
+in (match (_65_2325) with
+| (_65_2319, _65_2321, se, _65_2324) -> begin
 (
 
 let se = (match (se) with
-| FStar_Syntax_Syntax.Sig_inductive_typ (l, _65_2322, typars, k, [], [], quals, rng) -> begin
+| FStar_Syntax_Syntax.Sig_inductive_typ (l, _65_2328, typars, k, [], [], quals, rng) -> begin
 (
 
 let quals = if (FStar_All.pipe_right quals (FStar_List.contains FStar_Syntax_Syntax.Assumption)) then begin
@@ -3163,7 +3169,7 @@ quals
 end else begin
 (
 
-let _65_2331 = (let _160_904 = (FStar_Range.string_of_range rng)
+let _65_2337 = (let _160_904 = (FStar_Range.string_of_range rng)
 in (let _160_903 = (FStar_Syntax_Print.lid_to_string l)
 in (FStar_Util.print2 "%s (Warning): Adding an implicit \'assume new\' qualifier on %s\n" _160_904 _160_903)))
 in (FStar_Syntax_Syntax.Assumption)::(FStar_Syntax_Syntax.New)::quals)
@@ -3174,7 +3180,7 @@ let t = (match (typars) with
 | [] -> begin
 k
 end
-| _65_2336 -> begin
+| _65_2342 -> begin
 (let _160_907 = (let _160_906 = (let _160_905 = (FStar_Syntax_Syntax.mk_Total k)
 in ((typars), (_160_905)))
 in FStar_Syntax_Syntax.Tm_arrow (_160_906))
@@ -3182,7 +3188,7 @@ in (FStar_Syntax_Syntax.mk _160_907 None rng))
 end)
 in FStar_Syntax_Syntax.Sig_declare_typ (((l), ([]), (t), (quals), (rng)))))
 end
-| _65_2339 -> begin
+| _65_2345 -> begin
 se
 end)
 in (
@@ -3194,8 +3200,8 @@ end
 | (FStar_Parser_AST.TyconAbbrev (id, binders, kopt, t))::[] -> begin
 (
 
-let _65_2351 = (typars_of_binders env binders)
-in (match (_65_2351) with
+let _65_2357 = (typars_of_binders env binders)
+in (match (_65_2357) with
 | (env', typars) -> begin
 (
 
@@ -3205,7 +3211,7 @@ if (FStar_Util.for_some (fun _65_19 -> (match (_65_19) with
 | FStar_Syntax_Syntax.Effect -> begin
 true
 end
-| _65_2356 -> begin
+| _65_2362 -> begin
 false
 end)) quals) then begin
 FStar_Syntax_Syntax.teff
@@ -3225,7 +3231,7 @@ let quals = if (FStar_All.pipe_right quals (FStar_Util.for_some (fun _65_20 -> (
 | FStar_Syntax_Syntax.Logic -> begin
 true
 end
-| _65_2364 -> begin
+| _65_2370 -> begin
 false
 end)))) then begin
 quals
@@ -3253,7 +3259,7 @@ in (let _160_911 = (FStar_All.pipe_right quals (FStar_List.filter (fun _65_21 ->
 | FStar_Syntax_Syntax.Effect -> begin
 false
 end
-| _65_2372 -> begin
+| _65_2378 -> begin
 true
 end))))
 in ((_160_912), ([]), (typars), (c), (_160_911), (rng))))
@@ -3273,19 +3279,19 @@ let env = (FStar_Parser_Env.push_sigelt env se)
 in ((env), ((se)::[])))))))
 end))
 end
-| (FStar_Parser_AST.TyconRecord (_65_2378))::[] -> begin
+| (FStar_Parser_AST.TyconRecord (_65_2384))::[] -> begin
 (
 
 let trec = (FStar_List.hd tcs)
 in (
 
-let _65_2384 = (tycon_record_as_variant trec)
-in (match (_65_2384) with
+let _65_2390 = (tycon_record_as_variant trec)
+in (match (_65_2390) with
 | (t, fs) -> begin
 (desugar_tycon env rng ((FStar_Syntax_Syntax.RecordType (fs))::quals) ((t)::[]))
 end)))
 end
-| (_65_2388)::_65_2386 -> begin
+| (_65_2394)::_65_2392 -> begin
 (
 
 let env0 = env
@@ -3296,18 +3302,18 @@ in (
 
 let rec collect_tcs = (fun quals et tc -> (
 
-let _65_2399 = et
-in (match (_65_2399) with
+let _65_2405 = et
+in (match (_65_2405) with
 | (env, tcs) -> begin
 (match (tc) with
-| FStar_Parser_AST.TyconRecord (_65_2401) -> begin
+| FStar_Parser_AST.TyconRecord (_65_2407) -> begin
 (
 
 let trec = tc
 in (
 
-let _65_2406 = (tycon_record_as_variant trec)
-in (match (_65_2406) with
+let _65_2412 = (tycon_record_as_variant trec)
+in (match (_65_2412) with
 | (t, fs) -> begin
 (collect_tcs ((FStar_Syntax_Syntax.RecordType (fs))::quals) ((env), (tcs)) t)
 end)))
@@ -3315,29 +3321,29 @@ end
 | FStar_Parser_AST.TyconVariant (id, binders, kopt, constructors) -> begin
 (
 
-let _65_2418 = (desugar_abstract_tc quals env mutuals (FStar_Parser_AST.TyconAbstract (((id), (binders), (kopt)))))
-in (match (_65_2418) with
-| (env, _65_2415, se, tconstr) -> begin
+let _65_2424 = (desugar_abstract_tc quals env mutuals (FStar_Parser_AST.TyconAbstract (((id), (binders), (kopt)))))
+in (match (_65_2424) with
+| (env, _65_2421, se, tconstr) -> begin
 ((env), ((FStar_Util.Inl (((se), (constructors), (tconstr), (quals))))::tcs))
 end))
 end
 | FStar_Parser_AST.TyconAbbrev (id, binders, kopt, t) -> begin
 (
 
-let _65_2430 = (desugar_abstract_tc quals env mutuals (FStar_Parser_AST.TyconAbstract (((id), (binders), (kopt)))))
-in (match (_65_2430) with
-| (env, _65_2427, se, tconstr) -> begin
+let _65_2436 = (desugar_abstract_tc quals env mutuals (FStar_Parser_AST.TyconAbstract (((id), (binders), (kopt)))))
+in (match (_65_2436) with
+| (env, _65_2433, se, tconstr) -> begin
 ((env), ((FStar_Util.Inr (((se), (t), (quals))))::tcs))
 end))
 end
-| _65_2432 -> begin
+| _65_2438 -> begin
 (FStar_All.failwith "Unrecognized mutual type definition")
 end)
 end)))
 in (
 
-let _65_2435 = (FStar_List.fold_left (collect_tcs quals) ((env), ([])) tcs)
-in (match (_65_2435) with
+let _65_2441 = (FStar_List.fold_left (collect_tcs quals) ((env), ([])) tcs)
+in (match (_65_2441) with
 | (env, tcs) -> begin
 (
 
@@ -3345,12 +3351,12 @@ let tcs = (FStar_List.rev tcs)
 in (
 
 let tps_sigelts = (FStar_All.pipe_right tcs (FStar_List.collect (fun _65_23 -> (match (_65_23) with
-| FStar_Util.Inr (FStar_Syntax_Syntax.Sig_inductive_typ (id, uvs, tpars, k, _65_2443, _65_2445, _65_2447, _65_2449), t, quals) -> begin
+| FStar_Util.Inr (FStar_Syntax_Syntax.Sig_inductive_typ (id, uvs, tpars, k, _65_2449, _65_2451, _65_2453, _65_2455), t, quals) -> begin
 (
 
-let _65_2459 = (push_tparams env tpars)
-in (match (_65_2459) with
-| (env_tps, _65_2458) -> begin
+let _65_2465 = (push_tparams env tpars)
+in (match (_65_2465) with
+| (env_tps, _65_2464) -> begin
 (
 
 let t = (desugar_term env_tps t)
@@ -3359,25 +3365,25 @@ in (([]), (_160_922)))
 in (_160_923)::[]))
 end))
 end
-| FStar_Util.Inl (FStar_Syntax_Syntax.Sig_inductive_typ (tname, univs, tpars, k, mutuals, _65_2467, tags, _65_2470), constrs, tconstr, quals) -> begin
+| FStar_Util.Inl (FStar_Syntax_Syntax.Sig_inductive_typ (tname, univs, tpars, k, mutuals, _65_2473, tags, _65_2476), constrs, tconstr, quals) -> begin
 (
 
 let tycon = ((tname), (tpars), (k))
 in (
 
-let _65_2481 = (push_tparams env tpars)
-in (match (_65_2481) with
+let _65_2487 = (push_tparams env tpars)
+in (match (_65_2487) with
 | (env_tps, tps) -> begin
 (
 
-let data_tpars = (FStar_List.map (fun _65_2485 -> (match (_65_2485) with
-| (x, _65_2484) -> begin
+let data_tpars = (FStar_List.map (fun _65_2491 -> (match (_65_2491) with
+| (x, _65_2490) -> begin
 ((x), (Some (FStar_Syntax_Syntax.Implicit (true))))
 end)) tps)
 in (
 
-let _65_2511 = (let _160_935 = (FStar_All.pipe_right constrs (FStar_List.map (fun _65_2492 -> (match (_65_2492) with
-| (id, topt, _65_2490, of_notation) -> begin
+let _65_2517 = (let _160_935 = (FStar_All.pipe_right constrs (FStar_List.map (fun _65_2498 -> (match (_65_2498) with
+| (id, topt, _65_2496, of_notation) -> begin
 (
 
 let t = if of_notation then begin
@@ -3411,7 +3417,7 @@ let quals = (FStar_All.pipe_right tags (FStar_List.collect (fun _65_22 -> (match
 | FStar_Syntax_Syntax.RecordType (fns) -> begin
 (FStar_Syntax_Syntax.RecordConstructor (fns))::[]
 end
-| _65_2506 -> begin
+| _65_2512 -> begin
 []
 end))))
 in (
@@ -3426,13 +3432,13 @@ in ((tps), (_160_933)))
 in ((name), (_160_934))))))))
 end))))
 in (FStar_All.pipe_left FStar_List.split _160_935))
-in (match (_65_2511) with
+in (match (_65_2517) with
 | (constrNames, constrs) -> begin
 ((([]), (FStar_Syntax_Syntax.Sig_inductive_typ (((tname), (univs), (tpars), (k), (mutuals), (constrNames), (tags), (rng))))))::constrs
 end)))
 end)))
 end
-| _65_2513 -> begin
+| _65_2519 -> begin
 (FStar_All.failwith "impossible")
 end))))
 in (
@@ -3452,7 +3458,7 @@ let data_ops = (FStar_All.pipe_right tps_sigelts (FStar_List.collect (mk_data_pr
 in (
 
 let discs = (FStar_All.pipe_right sigelts (FStar_List.collect (fun _65_24 -> (match (_65_24) with
-| FStar_Syntax_Syntax.Sig_inductive_typ (tname, _65_2522, tps, k, _65_2526, constrs, quals, _65_2530) when ((FStar_List.length constrs) > (Prims.parse_int "1")) -> begin
+| FStar_Syntax_Syntax.Sig_inductive_typ (tname, _65_2528, tps, k, _65_2532, constrs, quals, _65_2536) when ((FStar_List.length constrs) > (Prims.parse_int "1")) -> begin
 (
 
 let quals = if (FStar_List.contains FStar_Syntax_Syntax.Abstract quals) then begin
@@ -3462,7 +3468,7 @@ quals
 end
 in (mk_data_discriminators quals env tname tps k constrs))
 end
-| _65_2535 -> begin
+| _65_2541 -> begin
 []
 end))))
 in (
@@ -3481,28 +3487,28 @@ end))))))))))
 
 let desugar_binders : FStar_Parser_Env.env  ->  FStar_Parser_AST.binder Prims.list  ->  (FStar_Parser_Env.env * FStar_Syntax_Syntax.binder Prims.list) = (fun env binders -> (
 
-let _65_2559 = (FStar_List.fold_left (fun _65_2544 b -> (match (_65_2544) with
+let _65_2565 = (FStar_List.fold_left (fun _65_2550 b -> (match (_65_2550) with
 | (env, binders) -> begin
 (match ((desugar_binder env b)) with
 | (Some (a), k) -> begin
 (
 
-let _65_2552 = (FStar_Parser_Env.push_bv env a)
-in (match (_65_2552) with
+let _65_2558 = (FStar_Parser_Env.push_bv env a)
+in (match (_65_2558) with
 | (env, a) -> begin
 (let _160_946 = (let _160_945 = (FStar_Syntax_Syntax.mk_binder (
 
-let _65_2553 = a
-in {FStar_Syntax_Syntax.ppname = _65_2553.FStar_Syntax_Syntax.ppname; FStar_Syntax_Syntax.index = _65_2553.FStar_Syntax_Syntax.index; FStar_Syntax_Syntax.sort = k}))
+let _65_2559 = a
+in {FStar_Syntax_Syntax.ppname = _65_2559.FStar_Syntax_Syntax.ppname; FStar_Syntax_Syntax.index = _65_2559.FStar_Syntax_Syntax.index; FStar_Syntax_Syntax.sort = k}))
 in (_160_945)::binders)
 in ((env), (_160_946)))
 end))
 end
-| _65_2556 -> begin
+| _65_2562 -> begin
 (Prims.raise (FStar_Syntax_Syntax.Error ((("Missing name in binder"), (b.FStar_Parser_AST.brange)))))
 end)
 end)) ((env), ([])) binders)
-in (match (_65_2559) with
+in (match (_65_2565) with
 | (env, binders) -> begin
 ((env), ((FStar_List.rev binders)))
 end)))
@@ -3516,8 +3522,8 @@ in (
 let monad_env = (FStar_Parser_Env.enter_monad_scope env eff_name)
 in (
 
-let _65_2573 = (desugar_binders monad_env eff_binders)
-in (match (_65_2573) with
+let _65_2579 = (desugar_binders monad_env eff_binders)
+in (match (_65_2579) with
 | (env, binders) -> begin
 (
 
@@ -3525,19 +3531,19 @@ let eff_k = (let _160_984 = (FStar_Parser_Env.default_total env)
 in (desugar_term _160_984 eff_kind))
 in (
 
-let _65_2584 = (FStar_All.pipe_right eff_decls (FStar_List.fold_left (fun _65_2577 decl -> (match (_65_2577) with
+let _65_2590 = (FStar_All.pipe_right eff_decls (FStar_List.fold_left (fun _65_2583 decl -> (match (_65_2583) with
 | (env, out) -> begin
 (
 
-let _65_2581 = (desugar_decl env decl)
-in (match (_65_2581) with
+let _65_2587 = (desugar_decl env decl)
+in (match (_65_2587) with
 | (env, ses) -> begin
 (let _160_988 = (let _160_987 = (FStar_List.hd ses)
 in (_160_987)::out)
 in ((env), (_160_988)))
 end))
 end)) ((env), ([]))))
-in (match (_65_2584) with
+in (match (_65_2590) with
 | (env, decls) -> begin
 (
 
@@ -3545,7 +3551,7 @@ let binders = (FStar_Syntax_Subst.close_binders binders)
 in (
 
 let actions = (FStar_All.pipe_right actions (FStar_List.map (fun d -> (match (d.FStar_Parser_AST.d) with
-| FStar_Parser_AST.Tycon (_65_2588, ((FStar_Parser_AST.TyconAbbrev (name, _65_2591, _65_2593, {FStar_Parser_AST.tm = FStar_Parser_AST.Construct (_65_2599, ((def, _65_2606))::((cps_type, _65_2602))::[]); FStar_Parser_AST.range = _65_2597; FStar_Parser_AST.level = _65_2595}), _65_2615))::[]) when (not (for_free)) -> begin
+| FStar_Parser_AST.Tycon (_65_2594, ((FStar_Parser_AST.TyconAbbrev (name, _65_2597, _65_2599, {FStar_Parser_AST.tm = FStar_Parser_AST.Construct (_65_2605, ((def, _65_2612))::((cps_type, _65_2608))::[]); FStar_Parser_AST.range = _65_2603; FStar_Parser_AST.level = _65_2601}), _65_2621))::[]) when (not (for_free)) -> begin
 (let _160_994 = (FStar_Parser_Env.qualify env name)
 in (let _160_993 = (let _160_990 = (desugar_term env def)
 in (FStar_Syntax_Subst.close binders _160_990))
@@ -3553,13 +3559,13 @@ in (let _160_992 = (let _160_991 = (desugar_typ env cps_type)
 in (FStar_Syntax_Subst.close binders _160_991))
 in {FStar_Syntax_Syntax.action_name = _160_994; FStar_Syntax_Syntax.action_unqualified_name = name; FStar_Syntax_Syntax.action_univs = []; FStar_Syntax_Syntax.action_defn = _160_993; FStar_Syntax_Syntax.action_typ = _160_992})))
 end
-| FStar_Parser_AST.Tycon (_65_2621, ((FStar_Parser_AST.TyconAbbrev (name, _65_2624, _65_2626, defn), _65_2631))::[]) when for_free -> begin
+| FStar_Parser_AST.Tycon (_65_2627, ((FStar_Parser_AST.TyconAbbrev (name, _65_2630, _65_2632, defn), _65_2637))::[]) when for_free -> begin
 (let _160_997 = (FStar_Parser_Env.qualify env name)
 in (let _160_996 = (let _160_995 = (desugar_term env defn)
 in (FStar_Syntax_Subst.close binders _160_995))
 in {FStar_Syntax_Syntax.action_name = _160_997; FStar_Syntax_Syntax.action_unqualified_name = name; FStar_Syntax_Syntax.action_univs = []; FStar_Syntax_Syntax.action_defn = _160_996; FStar_Syntax_Syntax.action_typ = FStar_Syntax_Syntax.tun}))
 end
-| _65_2637 -> begin
+| _65_2643 -> begin
 (Prims.raise (FStar_Syntax_Syntax.Error ((("Malformed action declaration; if this is an \"effect for free\", just provide the direct-style declaration. If this is not an \"effect for free\", please provide a pair of the definition and its cps-type with arrows inserted in the right place (see examples)."), (d.FStar_Parser_AST.drange)))))
 end))))
 in (
@@ -3661,15 +3667,15 @@ in (
 let env = (FStar_Parser_Env.enter_monad_scope env eff_name)
 in (
 
-let _65_2668 = (desugar_binders env eff_binders)
-in (match (_65_2668) with
+let _65_2674 = (desugar_binders env eff_binders)
+in (match (_65_2674) with
 | (env, binders) -> begin
 (
 
-let _65_2679 = (
+let _65_2685 = (
 
-let _65_2671 = (head_and_args defn)
-in (match (_65_2671) with
+let _65_2677 = (head_and_args defn)
+in (match (_65_2677) with
 | (head, args) -> begin
 (
 
@@ -3677,7 +3683,7 @@ let ed = (match (head.FStar_Parser_AST.tm) with
 | FStar_Parser_AST.Name (l) -> begin
 (FStar_Parser_Env.fail_or env (FStar_Parser_Env.try_lookup_effect_defn env) l)
 end
-| _65_2675 -> begin
+| _65_2681 -> begin
 (let _160_1054 = (let _160_1053 = (let _160_1052 = (let _160_1051 = (let _160_1050 = (FStar_Parser_AST.term_to_string head)
 in (Prims.strcat _160_1050 " not found"))
 in (Prims.strcat "Effect " _160_1051))
@@ -3688,23 +3694,23 @@ end)
 in (let _160_1055 = (desugar_args env args)
 in ((ed), (_160_1055))))
 end))
-in (match (_65_2679) with
+in (match (_65_2685) with
 | (ed, args) -> begin
 (
 
 let binders = (FStar_Syntax_Subst.close_binders binders)
 in (
 
-let sub = (fun _65_2685 -> (match (_65_2685) with
-| (_65_2683, x) -> begin
+let sub = (fun _65_2691 -> (match (_65_2691) with
+| (_65_2689, x) -> begin
 (
 
-let _65_2688 = (FStar_Syntax_Subst.open_term ed.FStar_Syntax_Syntax.binders x)
-in (match (_65_2688) with
+let _65_2694 = (FStar_Syntax_Subst.open_term ed.FStar_Syntax_Syntax.binders x)
+in (match (_65_2694) with
 | (edb, x) -> begin
 (
 
-let _65_2689 = if ((FStar_List.length args) <> (FStar_List.length edb)) then begin
+let _65_2695 = if ((FStar_List.length args) <> (FStar_List.length edb)) then begin
 (Prims.raise (FStar_Syntax_Syntax.Error ((("Unexpected number of arguments to effect constructor"), (defn.FStar_Parser_AST.range)))))
 end else begin
 ()
@@ -3786,7 +3792,7 @@ in (match (d.FStar_Parser_AST.d) with
 let se = FStar_Syntax_Syntax.Sig_pragma ((((trans_pragma p)), (d.FStar_Parser_AST.drange)))
 in ((env), ((se)::[])))
 end
-| FStar_Parser_AST.Fsdoc (_65_2711) -> begin
+| FStar_Parser_AST.Fsdoc (_65_2717) -> begin
 ((env), ([]))
 end
 | FStar_Parser_AST.TopLevelModule (id) -> begin
@@ -3805,8 +3811,8 @@ end
 | FStar_Parser_AST.Tycon (qual, tcs) -> begin
 (
 
-let tcs = (FStar_List.map (fun _65_2729 -> (match (_65_2729) with
-| (x, _65_2728) -> begin
+let tcs = (FStar_List.map (fun _65_2735 -> (match (_65_2735) with
+| (x, _65_2734) -> begin
 x
 end)) tcs)
 in (let _160_1094 = (FStar_List.map (trans_qual None) qual)
@@ -3816,29 +3822,29 @@ end
 (match ((let _160_1096 = (let _160_1095 = (desugar_term_maybe_top true env (FStar_Parser_AST.mk_term (FStar_Parser_AST.Let (((isrec), (lets), ((FStar_Parser_AST.mk_term (FStar_Parser_AST.Const (FStar_Const.Const_unit)) d.FStar_Parser_AST.drange FStar_Parser_AST.Expr))))) d.FStar_Parser_AST.drange FStar_Parser_AST.Expr))
 in (FStar_All.pipe_left FStar_Syntax_Subst.compress _160_1095))
 in _160_1096.FStar_Syntax_Syntax.n)) with
-| FStar_Syntax_Syntax.Tm_let (lbs, _65_2738) -> begin
+| FStar_Syntax_Syntax.Tm_let (lbs, _65_2744) -> begin
 (
 
 let fvs = (FStar_All.pipe_right (Prims.snd lbs) (FStar_List.map (fun lb -> (FStar_Util.right lb.FStar_Syntax_Syntax.lbname))))
 in (
 
 let quals = (match (quals) with
-| (_65_2746)::_65_2744 -> begin
+| (_65_2752)::_65_2750 -> begin
 (FStar_List.map (trans_qual None) quals)
 end
-| _65_2749 -> begin
+| _65_2755 -> begin
 (FStar_All.pipe_right (Prims.snd lbs) (FStar_List.collect (fun _65_25 -> (match (_65_25) with
-| {FStar_Syntax_Syntax.lbname = FStar_Util.Inl (_65_2760); FStar_Syntax_Syntax.lbunivs = _65_2758; FStar_Syntax_Syntax.lbtyp = _65_2756; FStar_Syntax_Syntax.lbeff = _65_2754; FStar_Syntax_Syntax.lbdef = _65_2752} -> begin
+| {FStar_Syntax_Syntax.lbname = FStar_Util.Inl (_65_2766); FStar_Syntax_Syntax.lbunivs = _65_2764; FStar_Syntax_Syntax.lbtyp = _65_2762; FStar_Syntax_Syntax.lbeff = _65_2760; FStar_Syntax_Syntax.lbdef = _65_2758} -> begin
 []
 end
-| {FStar_Syntax_Syntax.lbname = FStar_Util.Inr (fv); FStar_Syntax_Syntax.lbunivs = _65_2770; FStar_Syntax_Syntax.lbtyp = _65_2768; FStar_Syntax_Syntax.lbeff = _65_2766; FStar_Syntax_Syntax.lbdef = _65_2764} -> begin
+| {FStar_Syntax_Syntax.lbname = FStar_Util.Inr (fv); FStar_Syntax_Syntax.lbunivs = _65_2776; FStar_Syntax_Syntax.lbtyp = _65_2774; FStar_Syntax_Syntax.lbeff = _65_2772; FStar_Syntax_Syntax.lbdef = _65_2770} -> begin
 (FStar_Parser_Env.lookup_letbinding_quals env fv.FStar_Syntax_Syntax.fv_name.FStar_Syntax_Syntax.v)
 end))))
 end)
 in (
 
-let quals = if (FStar_All.pipe_right lets (FStar_Util.for_some (fun _65_2778 -> (match (_65_2778) with
-| (_65_2776, t) -> begin
+let quals = if (FStar_All.pipe_right lets (FStar_Util.for_some (fun _65_2784 -> (match (_65_2784) with
+| (_65_2782, t) -> begin
 (t.FStar_Parser_AST.level = FStar_Parser_AST.Formula)
 end)))) then begin
 (FStar_Syntax_Syntax.Logic)::quals
@@ -3853,11 +3859,11 @@ let lbs = if (FStar_All.pipe_right quals (FStar_List.contains FStar_Syntax_Synta
 let fv = (FStar_Util.right lb.FStar_Syntax_Syntax.lbname)
 in (
 
-let _65_2782 = lb
+let _65_2788 = lb
 in {FStar_Syntax_Syntax.lbname = FStar_Util.Inr ((
 
-let _65_2784 = fv
-in {FStar_Syntax_Syntax.fv_name = _65_2784.FStar_Syntax_Syntax.fv_name; FStar_Syntax_Syntax.fv_delta = FStar_Syntax_Syntax.Delta_abstract (fv.FStar_Syntax_Syntax.fv_delta); FStar_Syntax_Syntax.fv_qual = _65_2784.FStar_Syntax_Syntax.fv_qual})); FStar_Syntax_Syntax.lbunivs = _65_2782.FStar_Syntax_Syntax.lbunivs; FStar_Syntax_Syntax.lbtyp = _65_2782.FStar_Syntax_Syntax.lbtyp; FStar_Syntax_Syntax.lbeff = _65_2782.FStar_Syntax_Syntax.lbeff; FStar_Syntax_Syntax.lbdef = _65_2782.FStar_Syntax_Syntax.lbdef})))))
+let _65_2790 = fv
+in {FStar_Syntax_Syntax.fv_name = _65_2790.FStar_Syntax_Syntax.fv_name; FStar_Syntax_Syntax.fv_delta = FStar_Syntax_Syntax.Delta_abstract (fv.FStar_Syntax_Syntax.fv_delta); FStar_Syntax_Syntax.fv_qual = _65_2790.FStar_Syntax_Syntax.fv_qual})); FStar_Syntax_Syntax.lbunivs = _65_2788.FStar_Syntax_Syntax.lbunivs; FStar_Syntax_Syntax.lbtyp = _65_2788.FStar_Syntax_Syntax.lbtyp; FStar_Syntax_Syntax.lbeff = _65_2788.FStar_Syntax_Syntax.lbeff; FStar_Syntax_Syntax.lbdef = _65_2788.FStar_Syntax_Syntax.lbdef})))))
 in (((Prims.fst lbs)), (_160_1101)))
 end else begin
 lbs
@@ -3872,7 +3878,7 @@ in (
 let env = (FStar_Parser_Env.push_sigelt env s)
 in ((env), ((s)::[]))))))))
 end
-| _65_2791 -> begin
+| _65_2797 -> begin
 (FStar_All.failwith "Desugaring a let did not produce a let")
 end)
 end
@@ -3921,9 +3927,9 @@ end
 | FStar_Parser_AST.Exception (id, None) -> begin
 (
 
-let _65_2818 = (FStar_Parser_Env.fail_or env (FStar_Parser_Env.try_lookup_lid env) FStar_Syntax_Const.exn_lid)
-in (match (_65_2818) with
-| (t, _65_2817) -> begin
+let _65_2824 = (FStar_Parser_Env.fail_or env (FStar_Parser_Env.try_lookup_lid env) FStar_Syntax_Const.exn_lid)
+in (match (_65_2824) with
+| (t, _65_2823) -> begin
 (
 
 let l = (FStar_Parser_Env.qualify env id)
@@ -3986,8 +3992,8 @@ end
 | FStar_Parser_AST.KindAbbrev (id, binders, k) -> begin
 (
 
-let _65_2847 = (desugar_binders env binders)
-in (match (_65_2847) with
+let _65_2853 = (desugar_binders env binders)
+in (match (_65_2853) with
 | (env_k, binders) -> begin
 (
 
@@ -4039,7 +4045,7 @@ in (
 let dst = (lookup l.FStar_Parser_AST.mdest)
 in (
 
-let _65_2911 = (match (l.FStar_Parser_AST.lift_op) with
+let _65_2917 = (match (l.FStar_Parser_AST.lift_op) with
 | FStar_Parser_AST.NonReifiableLift (t) -> begin
 (let _160_1131 = (let _160_1130 = (let _160_1129 = (desugar_term env t)
 in (([]), (_160_1129)))
@@ -4061,7 +4067,7 @@ in (([]), (_160_1138)))
 in Some (_160_1139))
 in ((None), (_160_1140)))
 end)
-in (match (_65_2911) with
+in (match (_65_2917) with
 | (lift_wp, lift) -> begin
 (
 
@@ -4071,12 +4077,12 @@ end)))))
 end)))
 
 
-let desugar_decls : FStar_Parser_Env.env  ->  FStar_Parser_AST.decl Prims.list  ->  (FStar_Parser_Env.env * FStar_Syntax_Syntax.sigelts) = (fun env decls -> (FStar_List.fold_left (fun _65_2917 d -> (match (_65_2917) with
+let desugar_decls : FStar_Parser_Env.env  ->  FStar_Parser_AST.decl Prims.list  ->  (FStar_Parser_Env.env * FStar_Syntax_Syntax.sigelts) = (fun env decls -> (FStar_List.fold_left (fun _65_2923 d -> (match (_65_2923) with
 | (env, sigelts) -> begin
 (
 
-let _65_2921 = (desugar_decl env d)
-in (match (_65_2921) with
+let _65_2927 = (desugar_decl env d)
+in (match (_65_2927) with
 | (env, se) -> begin
 ((env), ((FStar_List.append sigelts se)))
 end))
@@ -4097,7 +4103,7 @@ end
 end)
 in (
 
-let _65_2944 = (match (m) with
+let _65_2950 = (match (m) with
 | FStar_Parser_AST.Interface (mname, decls, admitted) -> begin
 (let _160_1158 = (FStar_Parser_Env.prepare_module_or_interface true admitted env mname)
 in ((_160_1158), (mname), (decls), (true)))
@@ -4106,12 +4112,12 @@ end
 (let _160_1159 = (FStar_Parser_Env.prepare_module_or_interface false false env mname)
 in ((_160_1159), (mname), (decls), (false)))
 end)
-in (match (_65_2944) with
+in (match (_65_2950) with
 | ((env, pop_when_done), mname, decls, intf) -> begin
 (
 
-let _65_2947 = (desugar_decls env decls)
-in (match (_65_2947) with
+let _65_2953 = (desugar_decls env decls)
+in (match (_65_2953) with
 | (env, sigelts) -> begin
 (
 
@@ -4128,7 +4134,7 @@ let m = if (FStar_Options.interactive_fsi ()) then begin
 | FStar_Parser_AST.Module (mname, decls) -> begin
 FStar_Parser_AST.Interface (((mname), (decls), (true)))
 end
-| FStar_Parser_AST.Interface (mname, _65_2958, _65_2960) -> begin
+| FStar_Parser_AST.Interface (mname, _65_2964, _65_2966) -> begin
 (FStar_All.failwith (Prims.strcat "Impossible: " mname.FStar_Ident.ident.FStar_Ident.idText))
 end)
 end else begin
@@ -4136,24 +4142,24 @@ m
 end
 in (
 
-let _65_2968 = (desugar_modul_common curmod env m)
-in (match (_65_2968) with
-| (x, y, _65_2967) -> begin
+let _65_2974 = (desugar_modul_common curmod env m)
+in (match (_65_2974) with
+| (x, y, _65_2973) -> begin
 ((x), (y))
 end))))
 
 
 let desugar_modul : FStar_Parser_Env.env  ->  FStar_Parser_AST.modul  ->  (env_t * FStar_Syntax_Syntax.modul) = (fun env m -> (
 
-let _65_2974 = (desugar_modul_common None env m)
-in (match (_65_2974) with
+let _65_2980 = (desugar_modul_common None env m)
+in (match (_65_2980) with
 | (env, modul, pop_when_done) -> begin
 (
 
 let env = (FStar_Parser_Env.finish_module_or_interface env modul)
 in (
 
-let _65_2976 = if (FStar_Options.dump_module modul.FStar_Syntax_Syntax.name.FStar_Ident.str) then begin
+let _65_2982 = if (FStar_Options.dump_module modul.FStar_Syntax_Syntax.name.FStar_Ident.str) then begin
 (let _160_1170 = (FStar_Syntax_Print.modul_to_string modul)
 in (FStar_Util.print1 "%s\n" _160_1170))
 end else begin
@@ -4170,17 +4176,17 @@ end)))
 
 let desugar_file : FStar_Parser_Env.env  ->  FStar_Parser_AST.file  ->  (FStar_Parser_Env.env * FStar_Syntax_Syntax.modul Prims.list) = (fun env f -> (
 
-let _65_2989 = (FStar_List.fold_left (fun _65_2982 m -> (match (_65_2982) with
+let _65_2995 = (FStar_List.fold_left (fun _65_2988 m -> (match (_65_2988) with
 | (env, mods) -> begin
 (
 
-let _65_2986 = (desugar_modul env m)
-in (match (_65_2986) with
+let _65_2992 = (desugar_modul env m)
+in (match (_65_2992) with
 | (env, m) -> begin
 ((env), ((m)::mods))
 end))
 end)) ((env), ([])) f)
-in (match (_65_2989) with
+in (match (_65_2995) with
 | (env, mods) -> begin
 ((env), ((FStar_List.rev mods)))
 end)))
@@ -4188,15 +4194,15 @@ end)))
 
 let add_modul_to_env : FStar_Syntax_Syntax.modul  ->  FStar_Parser_Env.env  ->  FStar_Parser_Env.env = (fun m en -> (
 
-let _65_2994 = (FStar_Parser_Env.prepare_module_or_interface false false en m.FStar_Syntax_Syntax.name)
-in (match (_65_2994) with
+let _65_3000 = (FStar_Parser_Env.prepare_module_or_interface false false en m.FStar_Syntax_Syntax.name)
+in (match (_65_3000) with
 | (en, pop_when_done) -> begin
 (
 
 let en = (FStar_List.fold_left FStar_Parser_Env.push_sigelt (
 
-let _65_2995 = en
-in {FStar_Parser_Env.curmodule = Some (m.FStar_Syntax_Syntax.name); FStar_Parser_Env.curmonad = _65_2995.FStar_Parser_Env.curmonad; FStar_Parser_Env.modules = _65_2995.FStar_Parser_Env.modules; FStar_Parser_Env.open_namespaces = _65_2995.FStar_Parser_Env.open_namespaces; FStar_Parser_Env.modul_abbrevs = _65_2995.FStar_Parser_Env.modul_abbrevs; FStar_Parser_Env.sigaccum = _65_2995.FStar_Parser_Env.sigaccum; FStar_Parser_Env.localbindings = _65_2995.FStar_Parser_Env.localbindings; FStar_Parser_Env.recbindings = _65_2995.FStar_Parser_Env.recbindings; FStar_Parser_Env.sigmap = _65_2995.FStar_Parser_Env.sigmap; FStar_Parser_Env.default_result_effect = _65_2995.FStar_Parser_Env.default_result_effect; FStar_Parser_Env.iface = _65_2995.FStar_Parser_Env.iface; FStar_Parser_Env.admitted_iface = _65_2995.FStar_Parser_Env.admitted_iface; FStar_Parser_Env.expect_typ = _65_2995.FStar_Parser_Env.expect_typ}) m.FStar_Syntax_Syntax.exports)
+let _65_3001 = en
+in {FStar_Parser_Env.curmodule = Some (m.FStar_Syntax_Syntax.name); FStar_Parser_Env.curmonad = _65_3001.FStar_Parser_Env.curmonad; FStar_Parser_Env.modules = _65_3001.FStar_Parser_Env.modules; FStar_Parser_Env.open_namespaces = _65_3001.FStar_Parser_Env.open_namespaces; FStar_Parser_Env.modul_abbrevs = _65_3001.FStar_Parser_Env.modul_abbrevs; FStar_Parser_Env.sigaccum = _65_3001.FStar_Parser_Env.sigaccum; FStar_Parser_Env.localbindings = _65_3001.FStar_Parser_Env.localbindings; FStar_Parser_Env.recbindings = _65_3001.FStar_Parser_Env.recbindings; FStar_Parser_Env.sigmap = _65_3001.FStar_Parser_Env.sigmap; FStar_Parser_Env.default_result_effect = _65_3001.FStar_Parser_Env.default_result_effect; FStar_Parser_Env.iface = _65_3001.FStar_Parser_Env.iface; FStar_Parser_Env.admitted_iface = _65_3001.FStar_Parser_Env.admitted_iface; FStar_Parser_Env.expect_typ = _65_3001.FStar_Parser_Env.expect_typ}) m.FStar_Syntax_Syntax.exports)
 in (
 
 let env = (FStar_Parser_Env.finish_module_or_interface en m)
