src/ocaml-output/FStar_Syntax_Util.ml
@@ -5,7 +5,7 @@ let qual_id : FStar_Ident.lident  ->  FStar_Ident.ident  ->  FStar_Ident.lident 
 in (FStar_Ident.set_lid_range _133_5 id.FStar_Ident.idRange)))
 
 
-let mk_discriminator : FStar_Ident.lident  ->  FStar_Ident.lident = (fun lid -> (FStar_Ident.lid_of_ids (FStar_List.append lid.FStar_Ident.ns (((FStar_Ident.mk_ident (((Prims.strcat "is_" lid.FStar_Ident.ident.FStar_Ident.idText)), (lid.FStar_Ident.ident.FStar_Ident.idRange))))::[]))))
+let mk_discriminator : FStar_Ident.lident  ->  FStar_Ident.lident = (fun lid -> (FStar_Ident.lid_of_ids (FStar_List.append lid.FStar_Ident.ns (((FStar_Ident.mk_ident (((Prims.strcat FStar_Ident.reserved_prefix (Prims.strcat "is_" lid.FStar_Ident.ident.FStar_Ident.idText))), (lid.FStar_Ident.ident.FStar_Ident.idRange))))::[]))))
 
 
 let is_name : FStar_Ident.lident  ->  Prims.bool = (fun lid -> (
