examples/relational/new/ifc.fst
@@ -38,7 +38,7 @@ type low_equiv (env:label_fun) (h1:rel heap) =
 
 type ni_exp (env:label_fun) (e:exp) (l:label) = 
   forall (h: (rel heap)).
-   (low_equiv env h /\ is_Low l) ==> 
+   (low_equiv env h /\ Low? l) ==> 
      (interpret_exp (R?.r h) e = interpret_exp (R?.l h) e)
 
 (* env,pc:l |- c
@@ -47,31 +47,31 @@ type ni_exp (env:label_fun) (e:exp) (l:label) =
    - Low equivalent input heaps ==> Low equivalet output heaps 
 *)
 type ni_com' (env:label_fun) (c:com) (l:label) (h0:(rel (option heap))) = 
-    (is_Some (R?.l h0) /\ is_Some (R?.r h0) ==>
+    (Some? (R?.l h0) /\ Some? (R?.r h0) ==>
       (fun h0 -> 
       (fun o_l -> 
       (fun o_r -> 
-       ((is_Some o_l /\ is_Some o_r) 
+       ((Some? o_l /\ Some? o_r) 
         ==> (low_equiv env h0 
           ==> low_equiv env (R (Some?.v o_l) (Some?.v o_r)))))
         (interpret_com (R?.r h0) c))
         (interpret_com (R?.l h0) c))
         (R (Some?.v (R?.l h0)) (Some?.v (R?.r h0))))
     /\
-    (is_Some (R?.l h0) ==>
+    (Some? (R?.l h0) ==>
       (fun hl -> 
       (fun o_l -> 
         (forall r. (env r < l) 
-        ==> (is_Some o_l 
+        ==> (Some? o_l 
           ==> b2t (sel hl r = sel (Some?.v o_l) r))))
         (interpret_com hl c))
         ((Some?.v (R?.l h0))))
     /\
-    (is_Some (R?.r h0) ==>
+    (Some? (R?.r h0) ==>
       (fun hr -> 
       (fun o_r -> 
         (forall r. (env r < l) 
-        ==> (is_Some o_r 
+        ==> (Some? o_r 
           ==> b2t (sel hr r = sel (Some?.v o_r) r))))
         (interpret_com hr c))
         ((Some?.v (R?.r h0))))
