examples/relational/new/whilelanguage.fst
@@ -55,7 +55,7 @@ let decr h c =
   | _ ->   0
 
 (* Returns Some heap if the variant is correct *)
-val interpret_while : h:heap -> c:com{is_While c}
+val interpret_while : h:heap -> c:com{While? c}
   -> GTot (option heap) (decreases %[c; decr h c; 0])
 
 val interpret_com : h:heap -> c:com -> GTot (option heap) (decreases %[c; decr h c; 1])
@@ -105,7 +105,7 @@ let rec interpret_exp_st e =
 val interpret_com_st : c:com -> ST unit 
   (requires (fun _ -> True))
   (ensures  (fun h _ h' -> 
-    (fun o -> is_Some o ==> equal h' (Some?.v o)) 
+    (fun o -> Some? o ==> equal h' (Some?.v o)) 
       (interpret_com h c) ))
 let rec interpret_com_st c = 
   match c with
