ulib/FStar.Seq.fst
@@ -33,10 +33,10 @@ let index #a s i = List.index (MkSeq?.l s) i
 private val cons: #a:Type -> x:a -> s:seq a -> Tot (seq a)
 let cons #a x s = MkSeq (x::(MkSeq?.l s))
 
-private val hd: #a:Type -> s:seq a{is_Cons (MkSeq?.l s)} -> Tot a
+private val hd: #a:Type -> s:seq a{Cons? (MkSeq?.l s)} -> Tot a
 let hd #a s = List.hd (MkSeq?.l s)
 
-private val tl: #a:Type -> s:seq a{is_Cons (MkSeq?.l s)} -> Tot (seq a)
+private val tl: #a:Type -> s:seq a{Cons? (MkSeq?.l s)} -> Tot (seq a)
 let tl #a s = MkSeq (List.tl (MkSeq?.l s))
 
 abstract val create: #a:Type -> nat -> a -> Tot (seq a)
